theories/logic/sem_env.v
@@ -12,7 +12,13 @@ From hazel.program_logic Require Import weakest_precondition
 From affect.lib Require Import base.
 From affect.lang Require Import affect.
 From affect.logic Require Import sem_def.
+From affect.logic Require Import mode.
 From affect.logic Require Import sem_row.
+From affect.logic Require Import sem_types.
+
+Definition env_mbang {Σ} (m : mode) (Γ : env Σ) := map (λ xτ, (xτ.1, sem_ty_mbang m xτ.2)) Γ.
+
+Notation "![ m ] Γ" := (env_mbang m Γ) (at level 10) : sem_env_scope.
 
 Section env_lemmas_base.
   
@@ -24,7 +30,7 @@ Section env_lemmas_base.
   Lemma env_dom_nil :
     env_dom (Σ:= Σ) [] = [].
   Proof. done. Qed.
-  
+
   Lemma env_dom_cons x τ Γ :
     env_dom ((x, τ) :: Γ) = x :: env_dom Γ.
   Proof. done. Qed.
@@ -33,22 +39,22 @@ Section env_lemmas_base.
     env_dom (Γ₁ ++ Γ₂) = env_dom Γ₁ ++ env_dom Γ₂.
   Proof. by rewrite -map_app. Qed.
   
-  Lemma env_sem_typed_empty vs : ⟦ ([] : env Σ) ⟧ vs = True%I.
+  Lemma env_sem_typed_empty γ : ([] : env Σ) ⊨ₑ γ = True%I.
   Proof. done. Qed.
   
-  Lemma env_sem_typed_cons  x τ Γ' vs : 
-      ⟦ (x, τ) :: Γ' ⟧ vs = ((∃ v, ⌜ vs !! x = Some v ⌝ ∗ τ v) ∗ ⟦ Γ' ⟧ vs)%I.
+  Lemma env_sem_typed_cons  x τ Γ' γ : 
+    (x, τ) :: Γ' ⊨ₑ γ = ((∃ v, ⌜ γ !! x = Some v ⌝ ∗ τ v) ∗ Γ' ⊨ₑ γ)%I.
   Proof. done. Qed.
   
-  Lemma env_sem_typed_insert Γ vs (x : string) v :
+  Lemma env_sem_typed_insert Γ γ (x : string) v :
     x ∉ (env_dom Γ) →
-    ⟦ Γ ⟧ vs ⊣⊢ ⟦ Γ ⟧ (binder_insert x v vs).
+     Γ ⊨ₑ γ ⊣⊢  Γ ⊨ₑ (binder_insert x v γ).
   Proof.
     intros Helem. 
     iInduction Γ as [|[y τ] Γ'] "IH";
       first (iSplit; iIntros; by rewrite env_sem_typed_empty). 
     rewrite !env_sem_typed_cons; iSplit; iIntros "Henv";
-    iDestruct ("Henv") as "((%w & %Hvs & Hw) & HΓ')".
+    iDestruct ("Henv") as "((%w & %Hγ & Hw) & HΓ')".
     assert (x ≠ y).
     { rewrite env_dom_cons in Helem.
       destruct (not_elem_of_cons (env_dom Γ') x y) as [[ ] _]; done. }
@@ -63,20 +69,20 @@ Section env_lemmas_base.
       + iExists w.  iIntros "{$Hw} !%". 
         destruct (decide (y = x)) as [->|]. 
         { destruct Helem. rewrite env_dom_cons. apply elem_of_list_here. }
-        by rewrite lookup_insert_ne in Hvs.
+        by rewrite lookup_insert_ne in Hγ.
       + iApply "IH"; last done. iPureIntro. 
         destruct (not_elem_of_cons (env_dom Γ') x y) as [[ ] _]; done.
   Qed.
   
-  Lemma env_sem_typed_delete Γ vs (x : string) :
+  Lemma env_sem_typed_delete Γ γ (x : string) :
     x ∉ (env_dom Γ) →
-    ⟦ Γ ⟧ vs ⊣⊢ ⟦ Γ ⟧ (binder_delete x vs).
+     Γ ⊨ₑ γ ⊣⊢ Γ ⊨ₑ (binder_delete x γ).
   Proof.
     intros Helem. 
     iInduction Γ as [|[y τ] Γ'] "IH";
       first (iSplit; iIntros; by rewrite env_sem_typed_empty). 
     rewrite !env_sem_typed_cons; iSplit; iIntros "Henv";
-    iDestruct ("Henv") as "((%w & %Hvs & Hw) & HΓ')".
+    iDestruct ("Henv") as "((%w & %Hγ & Hw) & HΓ')".
     assert (x ≠ y).
     { rewrite env_dom_cons in Helem.
       destruct (not_elem_of_cons (env_dom Γ') x y) as [[ ] _]; done. }
@@ -89,14 +95,14 @@ Section env_lemmas_base.
       + iExists w.  iIntros "{$Hw} !%". 
         destruct (decide (y = x)) as [->|]. 
         { destruct Helem. rewrite env_dom_cons. apply elem_of_list_here. }
-        simpl in Hvs.
-        by rewrite lookup_delete_ne in Hvs.
+        simpl in Hγ.
+        by rewrite lookup_delete_ne in Hγ.
       + iApply "IH"; last done. iPureIntro. 
         destruct (not_elem_of_cons (env_dom Γ') x y) as [[ ] _]; done.
   Qed.
   
-  Lemma env_sem_typed_app Γ₁ Γ₂ vs :
-    ⟦ Γ₁ ++ Γ₂ ⟧ vs ⊣⊢ ⟦ Γ₁ ⟧ vs ∗ ⟦ Γ₂ ⟧ vs.
+  Lemma env_sem_typed_app Γ₁ Γ₂ γ :
+     Γ₁ ++ Γ₂ ⊨ₑ γ ⊣⊢  Γ₁ ⊨ₑ γ ∗ Γ₂ ⊨ₑ γ.
   Proof. 
     iInduction Γ₁ as [|[y τ] Γ₁'] "IH". 
     { iSplit; [iIntros; by iFrame|iIntros "[_ H] {$H}"]. }
@@ -140,8 +146,8 @@ Section env_lemmas_set_operations.
   Implicit Types Γ Γ₁ Γ₂ Γ₃ Δ : env Σ.
   Implicit Types τ τ₁ τ₂ : sem_ty Σ.
 
-  Lemma env_sem_typed_union Γ ws vs :
-    ⟦ Γ ⟧ vs ⊢ ⟦ Γ ⟧ (vs ∪ ws).
+  Lemma env_sem_typed_union Γ ws γ :
+     Γ ⊨ₑ γ ⊢  Γ ⊨ₑ (γ ∪ ws).
   Proof. 
     iIntros "HΓ". iInduction Γ as [|[x τ] Γ'] "IH"; first done.
     rewrite !env_sem_typed_cons.
@@ -152,9 +158,9 @@ Section env_lemmas_set_operations.
     by apply lookup_union_Some_l.
   Qed.
   
-  Lemma env_sem_typed_delete_union Γ Δ ws vs :
+  Lemma env_sem_typed_delete_union Γ Δ ws γ :
     env_dom Γ ⊆ env_dom Δ →
-    ⟦ Γ ⟧ vs ⊣⊢ ⟦ Γ ⟧ (delete (env_dom Δ) ws ∪ vs).
+     Γ ⊨ₑ γ ⊣⊢ Γ ⊨ₑ (delete (env_dom Δ) ws ∪ γ).
   Proof.
     intros ?. iSplit.
     - iInduction Γ as [|[x τ] Γ'] "IH"; first solve_env. 
@@ -180,8 +186,8 @@ Section env_lemmas_set_operations.
         iPureIntro. eapply subset_cons. by erewrite <- env_dom_cons.
   Qed.
   
-  Lemma env_sem_typed_difference_delete Γ Δ vs ws :
-    env_dom Γ ⊆ env_dom Δ → ⟦ Γ ⟧ vs ⊣⊢ ⟦ Γ ⟧ (vs ∖ delete (env_dom Δ) ws).
+  Lemma env_sem_typed_difference_delete Γ Δ γ ws :
+    env_dom Γ ⊆ env_dom Δ → Γ ⊨ₑ γ ⊣⊢ Γ ⊨ₑ (γ ∖ delete (env_dom Δ) ws).
   Proof.
     intros ?.
     iInduction Γ as [|[x τ] Γ'] "IH"; first (iSplit; solve_env).
@@ -205,8 +211,8 @@ Section env_lemmas_set_operations.
         iPureIntro. eapply subset_cons. by erewrite <- env_dom_cons.
   Qed.
   
-  Lemma env_sem_typed_delete_disjoint Γ Δ vs  :
-    env_dom Γ ## env_dom Δ → ⟦ Γ ⟧ vs ⊣⊢ ⟦ Γ ⟧ (delete (env_dom Δ) vs).
+  Lemma env_sem_typed_delete_disjoint Γ Δ γ  :
+    env_dom Γ ## env_dom Δ → Γ ⊨ₑ γ ⊣⊢ Γ ⊨ₑ (delete (env_dom Δ) γ).
   Proof. 
     iIntros (?).
     iInduction Γ as [|[x τ] Γ'] "IH"; first (iSplit; solve_env). 
@@ -226,8 +232,8 @@ Section env_lemmas_set_operations.
       + by iApply "IH".
   Qed. 
   
-  Lemma env_sem_typed_union_difference_delete Γ Δ vs ws :
-    env_dom Γ ## env_dom Δ → ⟦ Γ ⟧ (vs ∪ ws ∖ (delete (env_dom Δ) ws)) ⊢ ⟦ Γ ⟧ vs.
+  Lemma env_sem_typed_union_difference_delete Γ Δ γ ws :
+    env_dom Γ ## env_dom Δ → Γ ⊨ₑ (γ ∪ ws ∖ (delete (env_dom Δ) ws)) ⊢ Γ ⊨ₑ γ.
   Proof. 
     intros ?.
     iInduction Γ as [|[x τ] Γ'] "IH"; first solve_env.
@@ -245,33 +251,56 @@ Section env_lemmas_set_operations.
   
 End env_lemmas_set_operations.
 
-Section env_row_sub_typing.
+Section multi_env.
+  
+  Context `{heapGS Σ}.
 
-  Lemma row_env_sub_copy {Σ} (ρ : sem_row Σ) (Γ : env Σ) : 
-    copy_env Γ -∗ ρ ≼ₑ Γ.
-  Proof.
-    iIntros "#HΓcpy %vs %v %Φ !# Hρ HΓ.".
-    iDestruct ("HΓcpy" with "HΓ.") as "#HΓ".
-    iApply (pmono_prot_prop Σ ρ); last iApply "Hρ".  
-    iIntros "!# % $ //".
+  Class MultiE {Σ} (Γ : env Σ) := {
+    multi_env : ⊢ Γ ≤ₑ (![ MS ] Γ%E)
+  }.
+
+  Global Instance multi_env_persistent (Γ : env Σ) `{! MultiE Γ } :
+    ∀ γ, Persistent (Γ ⊨ₑ γ).
+  Proof. 
+    intros ?. rewrite /Persistent. iIntros "HΓ". 
+    inv MultiE0. iDestruct (multi_env0 with "HΓ") as "H!Γ". clear multi_env0.
+    iInduction Γ as [|[x τ] Γ'] "IH".
+    { iIntros "!# //". }
+    rewrite /env_mbang map_cons /= -/(env_mbang MS Γ').
+    iDestruct "H!Γ" as "(% & %Heq & Hτ. & HΓ'.)".
+    iDestruct ("IH" with "HΓ'.") as "#HΓ'".
+    rewrite /sem_ty_mbang /=. iDestruct "Hτ." as "#Hτ".
+    iModIntro. iExists v. iSplit; first done. iFrame "#".
   Qed.
 
-  Lemma row_env_sub_nil {Σ} (ρ : sem_row Σ) :    
-    ⊢ ρ ≼ₑ ([] : env Σ).
-  Proof. iApply row_env_sub_copy. iIntros "!# % _ //". Qed.
-
-  Lemma row_env_sub_cons {Σ} (ρ : sem_row Σ) x τ (Γ : env Σ) : 
-    ρ ≼ₑ Γ -∗ ρ ≼ₜ τ -∗ ρ ≼ₑ ((x, τ) :: Γ).
-  Proof.
-    iIntros "#HρΓ #Hρτ %vs %v %Φ !# Hρ (%w & %Heq & Hτ & HΓ)".
-    iSpecialize ("HρΓ" $! vs v Φ with "Hρ HΓ").
-    iSpecialize ("Hρτ" $! w v _ with "HρΓ Hτ").
-    iApply (pmono_prot_prop Σ ρ with "[] Hρτ"). 
-    iIntros "!# % [[$ HΓ] Hτ]".
-    iExists w. by iFrame.
+  Lemma multi_env_persistent_inv (Γ : env Σ) :
+    □ (∀ γ, Γ ⊨ₑ γ -∗ □ (Γ ⊨ₑ γ)) -∗ Γ ≤ₑ (![MS ] Γ).
+  Proof. 
+    iIntros "#H !# % HΓ.".
+    iDestruct ("H" with "HΓ.") as "#HΓ". iClear "HΓ. H".
+    iInduction Γ as [|[x τ] Γ'] "IH".
+    { rewrite /env_mbang //. }
+    rewrite /env_mbang map_cons /= -/(env_mbang MS Γ').
+    iDestruct "HΓ" as "(% & %Heq & Hτ. & HΓ'.)".
+    iDestruct ("IH" with "HΓ'.") as "#HΓ'".
+    rewrite /sem_ty_mbang /=. iDestruct "Hτ." as "#Hτ". simpl.
+    iExists v. iSplit; first done. iFrame "#".
   Qed.
 
-End env_row_sub_typing.
+  Global Instance multi_env_nil : @MultiE Σ [].
+  Proof. constructor. iIntros "!# % #$". Qed.
+  
+  Global Instance multi_env_cons (Γ : env Σ) x τ `{! MultiE Γ } `{! MultiT τ }:
+    MultiE ((x, τ) :: Γ).
+  Proof. 
+    constructor. iIntros "% !# (% & %Heq & #Hτ & #HΓ)".
+    iApply (multi_env_persistent_inv with "[]").
+    - iClear "Hτ HΓ". iIntros "!# % (% & %Heq' & #Hτ & #HΓ)". 
+      iModIntro. iExists v0. iSplit; first done. iFrame "#".
+    - iExists v. iSplit; first done. iFrame "#".
+  Qed.
+
+End multi_env.
 
 Section env_sub_typing.
 
@@ -280,43 +309,41 @@ Section env_sub_typing.
   Implicit Types Γ Γ₁ Γ₂ Γ₃ : env Σ.
   Implicit Types τ τ₁ τ₂ : sem_ty Σ.
 
-  Lemma env_le_refl Γ : ⊢ Γ ≤E Γ.
+  Lemma env_le_refl Γ : ⊢ Γ ≤ₑ Γ.
   Proof. iIntros "!# % $". Qed.
   
   Lemma env_le_trans Γ₁ Γ₂ Γ₃ : 
-    Γ₁ ≤E Γ₂ -∗
-    Γ₂ ≤E Γ₃ -∗
-    Γ₁ ≤E Γ₃.
+    Γ₁ ≤ₑ Γ₂ -∗
+    Γ₂ ≤ₑ Γ₃ -∗
+    Γ₁ ≤ₑ Γ₃.
   Proof.
-    iIntros "#HΓ₁₂ #HΓ₂₃ !# %vs HΓ₁ //=".  
+    iIntros "#HΓ₁₂ #HΓ₂₃ !# %γ HΓ₁ //=".  
     iApply "HΓ₂₃". by iApply "HΓ₁₂".
   Qed.
   
   Lemma env_le_cons Γ₁ Γ₂ τ₁ τ₂ x :
-    Γ₁ ≤E Γ₂ -∗
-    τ₁ ≤T τ₂ -∗
-    (x, τ₁) :: Γ₁ ≤E (x, τ₂) :: Γ₂.
+    Γ₁ ≤ₑ Γ₂ -∗
+    τ₁ ≤ₜ τ₂ -∗
+    (x, τ₁) :: Γ₁ ≤ₑ (x, τ₂) :: Γ₂.
   Proof.
-    iIntros "#HΓ₁₂ #Hτ₁₂ !# %vs [%v (Hlookup & Hv & HΓ₁)]".
+    iIntros "#HΓ₁₂ #Hτ₁₂ !# %γ [%v (Hlookup & Hv & HΓ₁)]".
     iExists v. iFrame. iSplitR "HΓ₁"; last (by iApply "HΓ₁₂").
     by iApply "Hτ₁₂".
   Qed.
   
-  Lemma env_le_copy_contraction Γ x τ :
-    copy_ty τ -∗
-    (x, τ) :: Γ ≤E (x, τ) :: (x, τ) :: Γ.
+  Lemma env_le_contraction Γ x τ `{! MultiT τ } :
+    ⊢ (x, τ) :: Γ ≤ₑ (x, τ) :: (x, τ) :: Γ.
   Proof.
-    iIntros "#Hcpy !# %vs".
-    iIntros "//= [%w (%Hrw & Hτ & HΓ)]". 
-    iDestruct ("Hcpy" with "Hτ") as "#Hτ'".
+    iIntros "!# %γ".
+    iIntros "//= [%w (%Hrw & #Hτ & HΓ)]". 
     by do 2 (iExists w; iFrame "%#").
   Qed.
   
   Lemma env_le_bring_forth Γ n x τ :
     nth_error Γ n = Some (x, τ) →
-    ⊢ Γ ≤E (x, τ) :: (list_delete n Γ) .
+    ⊢ Γ ≤ₑ (x, τ) :: (list_delete n Γ) .
   Proof.
-    iInduction n as [|] "IH" forall (Γ); iIntros (Hnth vs);
+    iInduction n as [|] "IH" forall (Γ); iIntros (Hnth γ);
     iIntros "!# HΓ"; simpl in Hnth; destruct Γ; first done; simplify_eq; first done.
     destruct p; simpl. rewrite !env_sem_typed_cons.
     iDestruct "HΓ" as "[$ HΓ]". rewrite -env_sem_typed_cons.
@@ -325,9 +352,9 @@ Section env_sub_typing.
   
   Lemma env_le_bring_forth_rev Γ n x τ :
     nth_error Γ n = Some (x, τ) →
-    ⊢ (x, τ) :: (list_delete n Γ) ≤E Γ.
+    ⊢ (x, τ) :: (list_delete n Γ) ≤ₑ Γ.
   Proof.
-    iInduction n as [|] "IH" forall (Γ); iIntros (Hnth vs);
+    iInduction n as [|] "IH" forall (Γ); iIntros (Hnth γ);
     simpl in Hnth; 
     destruct Γ as [|[y κ] Γ']; first done; 
     simplify_eq; simpl; first (iIntros "!# $").
@@ -337,28 +364,28 @@ Section env_sub_typing.
   Qed.
   
   Lemma env_le_swap_second Γ x y τ₁ τ₂ : 
-    ⊢ (y, τ₂) :: (x, τ₁) :: Γ ≤E (x, τ₁) :: (y, τ₂) :: Γ.
+    ⊢ (y, τ₂) :: (x, τ₁) :: Γ ≤ₑ (x, τ₁) :: (y, τ₂) :: Γ.
   Proof.
     pose proof (env_le_bring_forth_rev ((x, τ₁) :: (y, τ₂) :: Γ) 1 y τ₂).
     by apply H.
   Qed.
   
   Lemma env_le_swap_third Γ x y z τ₁ τ₂ τ₃: 
-    ⊢ (z, τ₃) :: (x, τ₁) :: (y, τ₂) :: Γ ≤E (x, τ₁) :: (y, τ₂) :: (z, τ₃) :: Γ.
+    ⊢ (z, τ₃) :: (x, τ₁) :: (y, τ₂) :: Γ ≤ₑ (x, τ₁) :: (y, τ₂) :: (z, τ₃) :: Γ.
   Proof.
     pose proof (env_le_bring_forth_rev ((x, τ₁) :: (y, τ₂) :: (z, τ₃) :: Γ) 2 z τ₃).
     by apply H.
   Qed.
   
   Lemma env_le_swap_fourth Γ x y z z' τ₁ τ₂ τ₃ τ₄: 
-    ⊢ (z', τ₄) :: (x, τ₁) :: (y, τ₂) :: (z, τ₃) :: Γ ≤E (x, τ₁) :: (y, τ₂) :: (z, τ₃) :: (z', τ₄) :: Γ.
+    ⊢ (z', τ₄) :: (x, τ₁) :: (y, τ₂) :: (z, τ₃) :: Γ ≤ₑ (x, τ₁) :: (y, τ₂) :: (z, τ₃) :: (z', τ₄) :: Γ.
   Proof.
     pose proof (env_le_bring_forth_rev ((x, τ₁) :: (y, τ₂) :: (z, τ₃) :: (z', τ₄) :: Γ) 3 z' τ₄).
     by apply H.
   Qed.
   
-  Lemma env_le_swap_env_singl Γ x τ : 
-    ⊢ (x, τ) :: Γ ≤E Γ ++ [(x, τ)].
+  Lemma env_le_swap_env_sing Γ x τ : 
+    ⊢ (x, τ) :: Γ ≤ₑ Γ ++ [(x, τ)].
   Proof.
     induction Γ as [|[y κ] Γ'].
     { simpl. iIntros "!# % $". }
@@ -369,7 +396,66 @@ Section env_sub_typing.
   Qed.
   
   Lemma env_le_weaken Γ x τ :
-    ⊢ (x, τ) :: Γ ≤E Γ.
+    ⊢ (x, τ) :: Γ ≤ₑ Γ.
   Proof. iIntros "!# % [% (? & ? & $)]". Qed.
 
 End env_sub_typing.
+
+Section row_env_sub.
+
+  Global Instance row_env_sub_nil {Σ} (ρ : sem_row Σ) : ρ ᵣ⪯ₑ ([] : env Σ).
+  Proof. 
+    constructor. iIntros "% % % !# Hρ _". 
+    iApply (pmono_prot_prop _ ρ with "[] Hρ").
+    iIntros "!# % $".
+  Qed.
+
+  Global Instance row_env_sub_cons {Σ} (ρ : sem_row Σ) x τ (Γ : env Σ) : 
+    ρ ᵣ⪯ₑ Γ → ρ ᵣ⪯ₜ τ → ρ ᵣ⪯ₑ ((x, τ) :: Γ).
+  Proof.
+    intros HρΓ Hρτ. constructor. 
+    iIntros "%γ %v %Φ !# Hρ (%w & %Heq & Hτ & HΓ)".
+    inv HρΓ. iDestruct (row_env_sub with "Hρ HΓ") as "HρΓ".
+    inv Hρτ. iDestruct (row_type_sub with "HρΓ Hτ") as "Hρτ".
+    iApply (pmono_prot_prop Σ ρ with "[] Hρτ"). 
+    iIntros "!# % [[$ HΓ] Hτ]".
+    iExists w. by iFrame.
+  Qed.
+
+  Global Instance row_env_sub_copy {Σ} (ρ : sem_row Σ) (Γ : env Σ) `{! MultiE Γ } : ρ ᵣ⪯ₑ Γ.
+  Proof.
+    constructor. iIntros "%γ %v %Φ !# Hρ #HΓ".
+    iApply (pmono_prot_prop Σ ρ); last iApply "Hρ".  
+    iIntros "!# % $ //".
+  Qed.
+
+End row_env_sub.
+
+Section mode_env_sub.
+
+  Global Instance mode_env_sub_nil {Σ} m : m ₘ⪯ₑ ([] : env Σ).
+  Proof. 
+    constructor. iIntros "% _". 
+    iApply bi.intuitionistically_intuitionistically_if. iIntros "!# //".
+  Qed.
+  
+  Global Instance mode_env_sub_cons {Σ} m x τ (Γ : env Σ) `{ m ₘ⪯ₑ Γ } `{ m ₘ⪯ₜ τ } : 
+    m ₘ⪯ₑ ((x, τ) :: Γ).
+  Proof.
+    constructor. iIntros "%γ (%w & %Heq & Hτ & HΓ)".
+    inv H. iDestruct (mode_env_sub with "HΓ") as "HmΓ".
+    inv H0. iDestruct (mode_type_sub with "Hτ") as "Hmτ".
+    iDestruct (bi.intuitionistically_if_sep_2 m (Γ ⊨ₑ γ) (τ w) with "[HmΓ Hmτ]") as "HmΓτ".
+    { iFrame. }
+    iApply (intuitionistically_if_mono_alt with "[] HmΓτ").
+    iIntros "!# [HΓ Hτ]". 
+    iExists w. by iFrame.
+  Qed.
+
+  Global Instance mode_env_sub_ms {Σ} m (Γ : env Σ) `{! MultiE Γ } : m ₘ⪯ₑ Γ.
+  Proof. 
+    constructor. iIntros "% #HΓ". 
+    by iApply bi.intuitionistically_intuitionistically_if.
+  Qed.
+
+End mode_env_sub.
