theories/logic/sem_row.v
@@ -49,20 +49,6 @@ Next Obligation.
   iIntros (??????) "(%op' & %v' & -> & H)". by iExists op', v'.
 Qed.
 
-Global Instance sem_row_cons_ne {Σ} op : NonExpansive2 (@sem_row_cons Σ op).
-Proof. 
-  intros ???????. rewrite /sem_row_cons. 
-  intros ??. simpl. do 7 f_equiv; first f_equiv; apply non_dep_fun_dist; by f_equiv.  
-Qed.
-Global Instance sem_row_cons_Proper {Σ} op : Proper ((≡) ==> (≡) ==> (≡)) (@sem_row_cons Σ op).
-Proof. apply ne_proper_2. apply _. Qed.
-
-Global Instance sem_row_cons_contractive {Σ} op n : Proper (dist_later n ==> dist n ==> dist n) (@sem_row_cons Σ op).
-Proof. 
-  intros ???????. rewrite /sem_row_cons. 
-  intros ?. simpl. do 6 f_equiv; first f_contractive; f_equiv; apply non_dep_fun_dist; by f_equiv.
-Qed.
-
 (* Recursive Row *)
 Definition sem_row_rec {Σ} (R : sem_row Σ → sem_row Σ) `{Contractive R} : sem_row Σ :=
   fixpoint R.
@@ -91,262 +77,293 @@ Next Obligation.
   iApply (sem_row_prop _ ρ with "Hρ").
 Qed.
 
-Global Instance sem_row_flip_mbang_ne {Σ} m : NonExpansive (@sem_row_flip_mbang Σ m).
-Proof. intros ?????. rewrite /sem_row_flip_mbang. intros ?. simpl. 
-       do 4 f_equiv. apply non_dep_fun_dist; by f_equiv. Qed.
-Global Instance sem_row_flip_bang_Proper {Σ} m : Proper ((≡) ==> (≡)) (@sem_row_flip_mbang Σ m).
-Proof. apply ne_proper. apply _. Qed.
-
-Global Instance sem_row_flip_mbang_rec_contractive {Σ} m (R : sem_row Σ -d> sem_row Σ) `{Contractive R} : 
-  Contractive (λ θ, sem_row_flip_mbang m (R θ)).
-Proof.
-  intros ??????. rewrite /sem_row_flip_mbang. simpl.
-  do 4 f_equiv. apply non_dep_fun_dist. by apply Contractive0.
-Qed. 
-
 (* Notations. *)
 Notation "⟨⟩" := (sem_row_nil) : sem_row_scope.
 Notation "opσ · ρ" := (sem_row_cons opσ.1%S opσ.2%S ρ%R) (at level 80, right associativity) : sem_row_scope.
-Notation "¡_[ m ] ρ" := (sem_row_flip_mbang m ρ) (at level 10) : sem_row_scope.
+Notation "¡[ m ] ρ" := (sem_row_flip_mbang m ρ) (at level 10) : sem_row_scope.
 Notation "'μR:' θ , ρ " := (sem_row_rec (λ θ, ρ%R)) (at level 50) : sem_row_scope.
 
-(* Subtyping on Rows *)
+Section row_properties.
 
-Lemma row_le_refl {Σ} (ρ : sem_row Σ) :
-  ⊢ ρ ≤R ρ.
-Proof. iApply iEff_le_refl. Qed.
+  Global Instance sem_row_cons_ne {Σ} op : NonExpansive2 (@sem_row_cons Σ op).
+  Proof. 
+    intros ???????. rewrite /sem_row_cons. 
+    intros ??. simpl. do 7 f_equiv; first f_equiv; apply non_dep_fun_dist; by f_equiv.  
+  Qed.
+  Global Instance sem_row_cons_Proper {Σ} op : Proper ((≡) ==> (≡) ==> (≡)) (@sem_row_cons Σ op).
+  Proof. apply ne_proper_2. apply _. Qed.
+  
+  Global Instance sem_row_cons_contractive {Σ} op n : Proper (dist_later n ==> dist n ==> dist n) (@sem_row_cons Σ op).
+  Proof. 
+    intros ???????. rewrite /sem_row_cons. 
+    intros ?. simpl. do 6 f_equiv; first f_contractive; f_equiv; apply non_dep_fun_dist; by f_equiv.
+  Qed.
+  
+  Global Instance sem_row_flip_mbang_ne {Σ} m : NonExpansive (@sem_row_flip_mbang Σ m).
+  Proof. intros ?????. rewrite /sem_row_flip_mbang. intros ?. simpl. 
+         do 4 f_equiv. apply non_dep_fun_dist; by f_equiv. Qed.
+  Global Instance sem_row_flip_bang_Proper {Σ} m : Proper ((≡) ==> (≡)) (@sem_row_flip_mbang Σ m).
+  Proof. apply ne_proper. apply _. Qed.
+  
+  Global Instance sem_row_flip_mbang_rec_contractive {Σ} m (R : sem_row Σ -d> sem_row Σ) `{Contractive R} : 
+    Contractive (λ θ, sem_row_flip_mbang m (R θ)).
+  Proof.
+    intros ??????. rewrite /sem_row_flip_mbang. simpl.
+    do 4 f_equiv. apply non_dep_fun_dist. by apply Contractive0.
+  Qed. 
 
-Lemma row_le_trans {Σ} (ρ₁ ρ₂ ρ₃ : sem_row Σ) :
-  ρ₁ ≤R ρ₂ -∗ 
-  ρ₂ ≤R ρ₃ -∗
-  ρ₁ ≤R ρ₃.
-Proof. iApply iEff_le_trans. Qed.
+End row_properties.
 
-Lemma row_le_nil {Σ} (ρ : sem_row Σ) : 
-  ⊢ ⟨⟩ ≤R ρ.
-Proof. iApply iEff_le_bottom. Qed.
+Section once_row.
 
-Lemma row_le_cons_comp {Σ} (ρ ρ' : sem_row Σ) (op : operation) (σ σ' : sem_sig Σ) : 
-  σ ≤S σ' -∗ ρ ≤R ρ' -∗ 
-  (op, σ) · ρ ≤R (op, σ') · ρ'.
-Proof.
-  iIntros "#Hσσ' #Hρρ'". rewrite /sem_row_cons /=. 
-  iIntros (??) "!# (%op' & %v' & -> & H)".
-  iExists op', v'; iSplit; first done.
-  destruct (decide (op = op')); first (by iApply "Hσσ'"). 
-  by iApply "Hρρ'".
-Qed.
+  (* Once Constraint *)
+  
+  Class OnceR {Σ} (ρ : sem_row Σ) := {
+    row_le_mfbang_elim : (⊢ (¡[ OS ] ρ%R) ≤ᵣ ρ%R)
+  }.
+  
+  Global Instance monoprot_once {Σ} (ρ : sem_row Σ) `{! OnceR ρ } : MonoProt ρ.
+  Proof.
+    constructor. iIntros (???) "HP Hρ".
+    inv OnceR0. iApply row_le_mfbang_elim0.
+    iExists Φ. simpl. iFrame.
+  Qed.
 
-Lemma row_le_swap_second {Σ} (op op' : operation) (σ σ' : sem_sig Σ) (ρ : sem_row Σ) : 
-  op ≠ op' →
-  ⊢ (op, σ) · (op', σ') · ρ ≤R (op', σ') · (op, σ) · ρ. 
-Proof. 
-  iIntros (Hneq). rewrite /sem_row_cons /=.
-  iIntros (??) "!# (%op'' & %v'' & %Heq & H)". simpl.
-  destruct (decide (op = op'')) as [->|].
-  - iExists op'', v''. iSplit; first done.
-    rewrite decide_False; last done.
-    iExists op'', v''; iSplit; first done.
-    rewrite decide_True //.
-  - iDestruct "H" as "(%op''' & %v''' & %Heq' & H)".
-    destruct (decide (op' = op''')) as [->|].
-    + iExists op'', v''; iSplit; first done.
-      simplify_eq. rewrite decide_True //.
-    + iExists op''', v''; iSplit; first by simplify_eq.
-      simplify_eq. rewrite decide_False //.
-      iExists op''', v'''. iSplit; first done.
-      rewrite decide_False //.
-Qed.
+End once_row.
 
-Corollary row_le_swap_third {Σ} (op op' op'' : operation) (σ σ' σ'' : sem_sig Σ) (ρ : sem_row Σ) : 
-  op ≠ op' → op' ≠ op'' → op'' ≠ op →
-  ⊢ (op, σ) · (op', σ') · (op'', σ'') · ρ ≤R (op'', σ'') · (op, σ) · (op', σ') · ρ. 
-Proof. 
-  iIntros (???). 
-  iApply row_le_trans; first iApply row_le_cons_comp; [iApply sig_le_refl|by iApply row_le_swap_second|].
-  by iApply row_le_swap_second.
-Qed.
+Section row_sub_typing.
 
-Corollary row_le_swap_fourth {Σ} (op op' op'' op''' : operation) (σ σ' σ'' σ''': sem_sig Σ) (ρ : sem_row Σ) : 
-  op ≠ op' → op ≠ op'' → op ≠ op''' → op' ≠ op'' → op' ≠ op''' → op'' ≠ op''' → 
-  ⊢ (op, σ) · (op', σ') · (op'', σ'') · (op''', σ''') · ρ ≤R 
-    (op''', σ''') · (op, σ) · (op', σ') · (op'', σ'') · ρ.
-Proof. 
-  iIntros (??????). 
-  iApply row_le_trans; first iApply row_le_cons_comp; [iApply sig_le_refl|by iApply row_le_swap_third|].
-  by iApply row_le_swap_second.
-Qed.
+  (* Subtyping on Rows *)
+  
+  Lemma row_le_refl {Σ} (ρ : sem_row Σ) :
+    ⊢ ρ ≤ᵣ ρ.
+  Proof. iApply iEff_le_refl. Qed.
+  
+  Lemma row_le_trans {Σ} (ρ₁ ρ₂ ρ₃ : sem_row Σ) :
+    ρ₁ ≤ᵣ ρ₂ -∗ 
+    ρ₂ ≤ᵣ ρ₃ -∗
+    ρ₁ ≤ᵣ ρ₃.
+  Proof. iApply iEff_le_trans. Qed.
+  
+  Lemma row_le_nil {Σ} (ρ : sem_row Σ) : 
+    ⊢ ⟨⟩ ≤ᵣ ρ.
+  Proof. iApply iEff_le_bottom. Qed.
+  
+  Lemma row_le_cons_comp {Σ} (ρ ρ' : sem_row Σ) (op : operation) (σ σ' : sem_sig Σ) : 
+    σ ≤ₛ σ' -∗ ρ ≤ᵣ ρ' -∗ 
+    (op, σ) · ρ ≤ᵣ (op, σ') · ρ'.
+  Proof.
+    iIntros "#Hσσ' #Hρρ'". rewrite /sem_row_cons /=. 
+    iIntros (??) "!# (%op' & %v' & -> & H)".
+    iExists op', v'; iSplit; first done.
+    destruct (decide (op = op')); first (by iApply "Hσσ'"). 
+    by iApply "Hρρ'".
+  Qed.
+  
+  Lemma row_le_swap_second {Σ} (op op' : operation) (σ σ' : sem_sig Σ) (ρ : sem_row Σ) : 
+    op ≠ op' →
+    ⊢ (op, σ) · (op', σ') · ρ ≤ᵣ (op', σ') · (op, σ) · ρ. 
+  Proof. 
+    iIntros (Hneq). rewrite /sem_row_cons /=.
+    iIntros (??) "!# (%op'' & %v'' & %Heq & H)". simpl.
+    destruct (decide (op = op'')) as [->|].
+    - iExists op'', v''. iSplit; first done.
+      rewrite decide_False; last done.
+      iExists op'', v''; iSplit; first done.
+      rewrite decide_True //.
+    - iDestruct "H" as "(%op''' & %v''' & %Heq' & H)".
+      destruct (decide (op' = op''')) as [->|].
+      + iExists op'', v''; iSplit; first done.
+        simplify_eq. rewrite decide_True //.
+      + iExists op''', v''; iSplit; first by simplify_eq.
+        simplify_eq. rewrite decide_False //.
+        iExists op''', v'''. iSplit; first done.
+        rewrite decide_False //.
+  Qed.
+  
+  Corollary row_le_swap_third {Σ} (op op' op'' : operation) (σ σ' σ'' : sem_sig Σ) (ρ : sem_row Σ) : 
+    op ≠ op' → op' ≠ op'' → op'' ≠ op →
+    ⊢ (op, σ) · (op', σ') · (op'', σ'') · ρ ≤ᵣ (op'', σ'') · (op, σ) · (op', σ') · ρ. 
+  Proof. 
+    iIntros (???). 
+    iApply row_le_trans; first iApply row_le_cons_comp; [iApply sig_le_refl|by iApply row_le_swap_second|].
+    by iApply row_le_swap_second.
+  Qed.
+  
+  Corollary row_le_swap_fourth {Σ} (op op' op'' op''' : operation) (σ σ' σ'' σ''': sem_sig Σ) (ρ : sem_row Σ) : 
+    op ≠ op' → op ≠ op'' → op ≠ op''' → op' ≠ op'' → op' ≠ op''' → op'' ≠ op''' → 
+    ⊢ (op, σ) · (op', σ') · (op'', σ'') · (op''', σ''') · ρ ≤ᵣ 
+      (op''', σ''') · (op, σ) · (op', σ') · (op'', σ'') · ρ.
+  Proof. 
+    iIntros (??????). 
+    iApply row_le_trans; first iApply row_le_cons_comp; [iApply sig_le_refl|by iApply row_le_swap_third|].
+    by iApply row_le_swap_second.
+  Qed.
+  
+  Lemma row_le_rec_unfold {Σ} (R : sem_row Σ → sem_row Σ) `{Contractive R} :
+    ⊢ (μR: θ, R θ) ≤ᵣ R (μR: θ, R θ).
+  Proof. rewrite {1} sem_row_rec_unfold //. iApply row_le_refl. Qed.
+  
+  Lemma row_le_rec_fold {Σ} (R : sem_row Σ → sem_row Σ) `{ Contractive R }:
+    ⊢ R (μR: θ, R θ) ≤ᵣ (μR: θ, R θ).
+  Proof. rewrite - {1} sem_row_rec_unfold. iApply row_le_refl. Qed.
+  
+  Lemma row_le_mfbang_intro {Σ} (m : mode) (ρ : sem_row Σ) :
+    ⊢ ρ ≤ᵣ ¡[ m ] ρ. 
+  Proof. 
+    rewrite /sem_row_flip_mbang. iIntros (??) "!# Hρ". simpl.
+    iExists Φ. iFrame. iApply bi.intuitionistically_intuitionistically_if. 
+    iIntros "!# % $ //".
+  Qed.
+  
+  Lemma row_le_mfbang_elim_ms {Σ} (ρ : sem_row Σ) :
+    ⊢ ¡[MS] ρ ≤ᵣ ρ. 
+  Proof. 
+    rewrite /sem_sig_flip_mbang. 
+    iIntros (v Φ) "!# (%Φ' & Hρ & HPost)". simpl.
+    by iApply (@pmono_prot_prop Σ ρ with "HPost").
+  Qed.
+  
+  Lemma row_le_mfbang_comp {Σ} m m' (ρ ρ' : sem_row Σ) :
+    m' ≤ₘ m -∗ ρ ≤ᵣ ρ' -∗
+    (¡[m] ρ) ≤ᵣ (¡[m'] ρ').
+  Proof. 
+    iIntros "#Hlem #Hleσ". destruct m.
+    - iDestruct (mode_le_OS_inv with "Hlem") as "->".
+      rewrite /row_le /sem_row_flip_mbang /tc_opaque.
+      by iApply iEff_le_upcl.
+    - iApply row_le_trans; first iApply row_le_mfbang_elim_ms. 
+      iApply row_le_trans; first iApply (row_le_mfbang_intro m').
+      rewrite /row_le /sem_row_flip_mbang /tc_opaque.
+      by iApply iEff_le_upcl.
+  Qed.
+  
+  Lemma row_le_mfbang_elim_cons {Σ} op m σ (ρ : sem_row Σ) :
+    ⊢ ¡[ m ] ((op, σ) · ρ) ≤ᵣ (op, ¡[ m ] σ)%S · (¡[ m ] ρ).
+  Proof. 
+    rewrite /sem_row_flip_mbang. 
+    iIntros (??) "!# (%Φ' & (%op' & %v' & -> & H) & Hpost)". simpl.
+    iExists op', v'. iSplit; first done.
+    destruct (decide (op = op')); first iNext; iExists Φ'; iFrame. 
+  Qed.
 
-Lemma row_le_rec_unfold {Σ} (R : sem_row Σ → sem_row Σ) `{Contractive R} :
-  ⊢ (μR: θ, R θ) ≤R R (μR: θ, R θ).
-Proof. rewrite {1} sem_row_rec_unfold //. iApply row_le_refl. Qed.
+  Global Instance row_cons_once {Σ} (ρ : sem_row Σ) op (σ : sem_sig Σ) `{! OnceS σ, ! OnceR ρ } :
+    OnceR ((op, σ) · ρ)%R.
+  Proof.
+    constructor. inv OnceS0. inv OnceR0.
+    iApply row_le_trans; first iApply row_le_mfbang_elim_cons.
+    iApply row_le_cons_comp; [iApply sig_le_mfbang_elim|iApply row_le_mfbang_elim0].
+  Qed.
+  
+  Lemma row_le_mfbang_idemp {Σ} m (ρ : sem_row Σ) :
+    ⊢ (¡[ m ] (¡[ m ] ρ)) ≤ᵣ ((¡[ m ] ρ)).
+  Proof. 
+    iIntros (v Φ) "!# (%Φ' & (%Φ'' & H & HPost') & HPost)". 
+    rewrite /sem_row_flip_mbang /=.
+    iDestruct (bi.intuitionistically_if_sep_2 with "[HPost HPost']") as "HP"; first iFrame.
+    iExists Φ''. iFrame.
+    iApply (bi.intuitionistically_if_mono with "HP").
+    iIntros "[H1 H2] % HΦ''". iApply ("H2" with "[H1 HΦ'']"). 
+    by iApply "H1".
+  Qed.
 
-Lemma row_le_rec_fold {Σ} (R : sem_row Σ → sem_row Σ) `{ Contractive R }:
-  ⊢ R (μR: θ, R θ) ≤R (μR: θ, R θ).
-Proof. rewrite - {1} sem_row_rec_unfold. iApply row_le_refl. Qed.
+  Global Instance row_fbang_once {Σ} (ρ : sem_row Σ) : OnceR (¡[OS] ρ)%R.
+  Proof. constructor. iApply row_le_mfbang_idemp. Qed.
+  
+  Lemma row_le_mfbang_comm {Σ} m m' (ρ : sem_row Σ) :
+    ⊢ (¡[ m ] (¡[ m' ] ρ)) ≤ᵣ (¡[ m' ] (¡[ m ] ρ)).
+  Proof. 
+    destruct m, m'.
+    - iApply row_le_refl.
+    - iApply row_le_trans; first iApply row_le_mfbang_comp.
+      { iApply mode_le_refl. }
+      { iApply row_le_mfbang_elim_ms. }
+      iApply row_le_mfbang_intro.
+    - iApply row_le_trans; first iApply row_le_mfbang_elim_ms.
+      iApply row_le_mfbang_comp; first iApply mode_le_refl. iApply row_le_mfbang_intro.
+    - iApply row_le_refl.
+  Qed.
+  
+  Lemma row_le_mfbang_elim_nil {Σ} m :
+     ⊢ ¡[m] ⟨⟩%R ≤ᵣ (⟨⟩%R : sem_row Σ).
+  Proof. 
+    destruct m; simpl; last iApply row_le_mfbang_elim_ms.
+    iIntros (??) "!# (% & [] & _)".
+  Qed.
+  
+  Global Instance row_nil_once {Σ} : OnceR (⟨⟩ : sem_row Σ)%R.
+  Proof. constructor. iApply row_le_mfbang_elim_nil. Qed.
+  
+  Lemma row_le_mfbang_elim_rec {Σ} (m : mode) (R : sem_row Σ → sem_row Σ) `{ Contractive R }: 
+    (∀ θ, ¡[ m ] (R θ) ≤ᵣ (R θ)) -∗ ¡[ m ] (μR: θ, R θ) ≤ᵣ (μR: θ, R θ).
+  Proof. 
+    iIntros "#Hle". destruct m; last iApply row_le_mfbang_elim_ms.
+    iIntros (??) "!# (%Φ' & H & HP)". simpl.
+    iApply sem_row_rec_unfold_iEff. rewrite sem_row_rec_unfold_iEff.
+    iApply "Hle". iExists Φ'. simpl. iFrame.
+  Qed.
+  
+  Global Instance row_rec_once {Σ} (R : sem_row Σ → sem_row Σ) `{Contractive R} :
+    (∀ θ, OnceR (R θ)) → OnceR (μR: θ, R θ)%R.
+  Proof.
+    intros H. constructor. 
+    iApply row_le_mfbang_elim_rec. iIntros (θ). 
+    destruct (H θ). iApply row_le_mfbang_elim0.
+  Qed.
 
-Lemma row_le_mfbang_intro {Σ} (m : mode) (ρ : sem_row Σ) :
-  ⊢ ρ ≤R ¡_[ m ] ρ. 
-Proof. 
-  rewrite /sem_row_flip_mbang. iIntros (??) "!# Hρ". simpl.
-  iExists Φ. iFrame. iApply bi.intuitionistically_intuitionistically_if. 
-  iIntros "!# % $ //".
-Qed.
+End row_sub_typing.
+  
+Section row_type_sub.
 
-Lemma row_le_mfbang_elim_ms {Σ} (ρ : sem_row Σ) :
-  ⊢ ¡_[MS] ρ ≤R ρ. 
-Proof. 
-  rewrite /sem_sig_flip_mbang. 
-  iIntros (v Φ) "!# (%Φ' & Hρ & HPost)". simpl.
-  by iApply (@pmono_prot_prop Σ ρ with "HPost").
-Qed.
+  (* Substructurality relation on rows wrt to types and environments *)
+  
+  Definition mono_prot_on_prop {Σ} (Ψ : iEff Σ) (P : iProp Σ) : iProp Σ :=
+    □ (∀ v Φ, iEff_car Ψ v Φ -∗ P -∗ iEff_car Ψ v (λ w, Φ w ∗ P))%I.
+  
+  (* For semantic signatures, being monotonic on all propositions is the same as being monotonic
+     because semantic signatures are persistently monotonic by definition *)
+  Lemma mono_prot_on_prop_monotonic {Σ} (σ : sem_sig Σ) : 
+    (⊢ ∀ P, mono_prot_on_prop σ P) ↔ MonoProt σ.
+  Proof.
+    split.
+    - iIntros (H). constructor. iIntros (v Φ Φ') "Hpost HΨ".
+      iDestruct (H with "HΨ Hpost") as "H".
+      iApply (pmono_prot_prop _ σ with "[] H").
+      { iIntros "!# % [HΦ HPost]". by iApply "HPost". }
+    - iIntros (H) "%P %v %Φ !# Hσ HP". inv H.
+      iApply (monotonic_prot with "[HP] Hσ"). iIntros (?) "$ //".
+  Qed.
+  
+  Class RowTypeSub {Σ} (ρ : sem_row Σ) (τ : sem_ty Σ) := {
+    row_type_sub : ⊢ (∀ v, mono_prot_on_prop ρ (τ v))
+  }.
+  
+  Global Instance row_type_sub_once {Σ} (ρ : sem_row Σ) (τ : sem_ty Σ) `{! OnceR ρ} : RowTypeSub ρ τ.
+  Proof.
+    constructor.
+    iIntros (w v Φ) "!# Hρ Hτ". 
+    iApply (monotonic_prot v Φ (λ w', Φ w' ∗ τ w)%I with "[Hτ] Hρ").
+    iIntros "% $ //".
+  Qed.
+  
+End row_type_sub.
 
-Lemma row_le_mfbang_comp {Σ} m m' (ρ ρ' : sem_row Σ) :
-  m' ≤M m -∗ ρ ≤R ρ' -∗
-  (¡_[m] ρ) ≤R (¡_[m'] ρ').
-Proof. 
-  iIntros "#Hlem #Hleσ". destruct m.
-  - iDestruct (mode_le_OS_inv with "Hlem") as "->".
-    rewrite /row_le /sem_row_flip_mbang /tc_opaque.
-    by iApply iEff_le_upcl.
-  - iApply row_le_trans; first iApply row_le_mfbang_elim_ms. 
-    iApply row_le_trans; first iApply (row_le_mfbang_intro m').
-    rewrite /row_le /sem_row_flip_mbang /tc_opaque.
-    by iApply iEff_le_upcl.
-Qed.
+Section row_env_sub.
 
-Lemma row_le_mfbang_cons {Σ} op m σ (ρ : sem_row Σ) :
-  ⊢ ¡_[ m ] ((op, σ) · ρ) ≤R (op, ¡_[ m ] σ)%S · (¡_[ m ] ρ).
-Proof. 
-  rewrite /sem_row_flip_mbang. 
-  iIntros (??) "!# (%Φ' & (%op' & %v' & -> & H) & Hpost)". simpl.
-  iExists op', v'. iSplit; first done.
-  destruct (decide (op = op')); first iNext; iExists Φ'; iFrame. 
-Qed.
+  Class RowEnvSub {Σ} (ρ : sem_row Σ) (Γ : env Σ) := {
+    row_env_sub : ⊢ (∀ γ, mono_prot_on_prop ρ (Γ ⊨ₑ γ))
+  }.
+  
+  Global Instance row_env_sub_once {Σ} (ρ : sem_row Σ) (Γ : env Σ) `{! OnceR ρ} : RowEnvSub ρ Γ.
+  Proof.
+    constructor.
+    iIntros (γ v Φ) "!# Hρ HΓ".
+    iApply (monotonic_prot v Φ (λ w', Φ w' ∗ Γ ⊨ₑ γ)%I with "[HΓ] Hρ").
+    iIntros "% $ //".
+  Qed.
+  
+End row_env_sub.
 
-Lemma row_le_mfbang_idemp {Σ} m (ρ : sem_row Σ) :
-  ⊢ (¡_[ m ] (¡_[ m ] ρ)) ≤R ((¡_[ m ] ρ)).
-Proof. 
-  iIntros (v Φ) "!# (%Φ' & (%Φ'' & H & HPost') & HPost)". 
-  rewrite /sem_row_flip_mbang /=.
-  iDestruct (bi.intuitionistically_if_sep_2 with "[HPost HPost']") as "HP"; first iFrame.
-  iExists Φ''. iFrame.
-  iApply (bi.intuitionistically_if_mono with "HP").
-  iIntros "[H1 H2] % HΦ''". iApply ("H2" with "[H1 HΦ'']"). 
-  by iApply "H1".
-Qed.
-
-Lemma row_le_mfbang_comm {Σ} m m' (ρ : sem_row Σ) :
-  ⊢ (¡_[ m ] (¡_[ m' ] ρ)) ≤R (¡_[ m' ] (¡_[ m ] ρ)).
-Proof. 
-  destruct m, m'.
-  - iApply row_le_refl.
-  - iApply row_le_trans; first iApply row_le_mfbang_comp.
-    { iApply mode_le_refl. }
-    { iApply row_le_mfbang_elim_ms. }
-    iApply row_le_mfbang_intro.
-  - iApply row_le_trans; first iApply row_le_mfbang_elim_ms.
-    iApply row_le_mfbang_comp; first iApply mode_le_refl. iApply row_le_mfbang_intro.
-  - iApply row_le_refl.
-Qed.
-
-Lemma row_le_mfbang_nil {Σ} m :
-   ⊢ ¡_[m] ⟨⟩%R ≤R (⟨⟩%R : sem_row Σ).
-Proof. 
-  destruct m; simpl; last iApply row_le_mfbang_elim_ms.
-  iIntros (??) "!# (% & [] & _)".
-Qed.
-
-Lemma row_le_mfbang_rec {Σ} (m : mode) (R : sem_row Σ → sem_row Σ) `{ Contractive R }: 
-  (∀ θ, ¡_[ m ] (R θ) ≤R (R θ)) -∗ ¡_[ m ] (μR: θ, R θ) ≤R (μR: θ, R θ).
-Proof. 
-  iIntros "#Hle". destruct m; last iApply row_le_mfbang_elim_ms.
-  iIntros (??) "!# (%Φ' & H & HP)". simpl.
-  iApply sem_row_rec_unfold_iEff. rewrite sem_row_rec_unfold_iEff.
-  iApply "Hle". iExists Φ'. simpl. iFrame.
-Qed.
-
-(* Once Constraint *)
-
-Class OnceR {Σ} (ρ : sem_row Σ) := {
-  flip_mbang_elim : (⊢ (¡_[ OS ] ρ%R) ≤R ρ%R)
-}.
-
-Global Instance row_nil_once {Σ} : OnceR (⟨⟩ : sem_row Σ)%R.
-Proof. constructor. iApply row_le_mfbang_nil. Qed.
-
-Global Instance row_cons_once {Σ} (ρ : sem_row Σ) op (σ : sem_sig Σ) `{! OnceS σ, ! OnceR ρ } :
-  OnceR ((op, σ) · ρ)%R.
-Proof.
-  constructor. inv OnceS0. inv OnceR0.
-  iApply row_le_trans; first iApply row_le_mfbang_cons.
-  iApply row_le_cons_comp; [iApply flip_mbang_elim0|iApply flip_mbang_elim1].
-Qed.
-
-Global Instance row_fbang_once {Σ} (ρ : sem_row Σ) : OnceR (¡_[OS] ρ)%R.
-Proof. constructor. iApply row_le_mfbang_idemp. Qed.
-
-Global Instance row_rec_once {Σ} (R : sem_row Σ → sem_row Σ) `{Contractive R} :
-  (∀ θ, OnceR (R θ)) → OnceR (μR: θ, R θ)%R.
-Proof.
-  intros H. constructor. 
-  iApply row_le_mfbang_rec. iIntros (θ). 
-  destruct (H θ). iApply flip_mbang_elim0.
-Qed.
-
-Global Instance monoprot_once {Σ} (ρ : sem_row Σ) `{! OnceR ρ } : MonoProt ρ.
-Proof.
-  constructor. iIntros (???) "HP Hρ".
-  inv OnceR0. iApply flip_mbang_elim0.
-  iExists Φ. simpl. iFrame.
-Qed.
-
-(* Substructurality relation on rows wrt to types and environments *)
-
-Definition mono_prot_on_prop {Σ} (Ψ : iEff Σ) (P : iProp Σ) : iProp Σ :=
-  □ (∀ v Φ, iEff_car Ψ v Φ -∗ P -∗ iEff_car Ψ v (λ w, Φ w ∗ P))%I.
-
-(* For semantic signatures, being monotonic on all propositions is the same as being monotonic
-   because semantic signatures are persistently monotonic by definition *)
-Lemma mono_prot_on_prop_monotonic {Σ} (σ : sem_sig Σ) : 
-  (⊢ ∀ P, mono_prot_on_prop σ P) ↔ MonoProt σ.
-Proof.
-  split.
-  - iIntros (H). constructor. iIntros (v Φ Φ') "Hpost HΨ".
-    iDestruct (H with "HΨ Hpost") as "H".
-    iApply (pmono_prot_prop _ σ with "[] H").
-    { iIntros "!# % [HΦ HPost]". by iApply "HPost". }
-  - iIntros (H) "%P %v %Φ !# Hσ HP". inv H.
-    iApply (monotonic_prot with "[HP] Hσ"). iIntros (?) "$ //".
-Qed.
-
-Definition row_type_sub {Σ} (ρ : sem_row Σ) (τ : sem_ty Σ) : iProp Σ := 
-  (∀ v, mono_prot_on_prop ρ (τ v)).
-
-Notation "ρ ≼ₜ τ" := (row_type_sub ρ%R τ%T)%I (at level 80) : bi_scope.
-
-Lemma row_type_sub_once {Σ} (ρ : sem_row Σ) (τ : sem_ty Σ) `{! OnceR ρ} : ⊢ ρ ≼ₜ τ.
-Proof.
-  iIntros (w v Φ) "!# Hρ Hτ". 
-  iApply (monotonic_prot v Φ (λ w', Φ w' ∗ τ w)%I with "[Hτ] Hρ").
-  iIntros "% $ //".
-Qed.
-
-Lemma row_type_sub_fbang {Σ} (ρ : sem_row Σ) (τ : sem_ty Σ) : ⊢ (¡_[OS] ρ) ≼ₜ τ.
-Proof. iApply row_type_sub_once. Qed.
-
-Definition row_env_sub {Σ} (ρ : sem_row Σ) (Γ : env Σ) : iProp Σ := 
-  (∀ vs, mono_prot_on_prop ρ (⟦ Γ ⟧ vs)).
-
-Notation "ρ ≼ₑ Γ" := (row_env_sub ρ%R Γ%T) (at level 80) : bi_scope.
-
-Lemma row_env_sub_once {Σ} (ρ : sem_row Σ) (Γ : env Σ) `{! OnceR ρ} : ⊢ ρ ≼ₑ Γ.
-Proof.
-  iIntros (γ v Φ) "!# Hρ HΓ".
-  iApply (monotonic_prot v Φ (λ w', Φ w' ∗ ⟦ Γ ⟧ γ)%I with "[HΓ] Hρ").
-  iIntros "% $ //".
-Qed.
-
-Lemma row_env_sub_fbang {Σ} (ρ : sem_row Σ) (Γ : env Σ) : ⊢ (¡_[OS] ρ) ≼ₑ Γ.
-Proof. iApply row_env_sub_once. Qed.
-
+(* Notations *)
+Notation "ρ ᵣ⪯ₑ Γ" := (RowEnvSub ρ%R Γ%T) (at level 80).
+Notation "ρ ᵣ⪯ₜ τ" := (RowTypeSub ρ%R τ%T)%I (at level 80).
