theories/logic/sem_sig.v
@@ -41,6 +41,67 @@ Proof.
   rewrite (iEff_tele_eq' [tele _] [tele _]) //. 
 Qed.
 
+(* Flip-Bang Signature *)
+Program Definition sem_sig_flip_mbang {Σ} (m : mode) (σ : sem_sig Σ) : sem_sig Σ := @PMonoProt Σ (upcl m σ) _.
+Next Obligation.
+  iIntros (??????) "#HΦ Hσ". 
+  destruct m.
+  - pose proof (upcl_mono_prot σ) as []. 
+    iApply (monotonic_prot with "HΦ Hσ").
+  - pose proof (pers_upcl_pers_mono_prot σ) as [].
+    iApply (pers_monotonic_prot with "HΦ Hσ").
+Qed.
+
+(* Notations. *)
+Notation "'∀S..:' tt , κ '=>' ι" := 
+  (sem_sig_eff (λ tt, κ%T) (λ tt, ι%T))
+  (at level 200, tt binder, right associativity,
+   format "'[ ' '∀S..:' tt ,  κ  =>  ι  ']'") : sem_sig_scope.
+
+Notation "'∀S:' x .. y , κ '=>' ι" := 
+  (sem_sig_eff 
+  (@tele_app ((TeleS (λ x, .. (TeleS (λ y, TeleO)) ..))) (sem_ty _) (λ x, .. (λ y, κ%T) ..)) 
+  (@tele_app ((TeleS (λ x, .. (TeleS (λ y, TeleO)) ..))) (sem_ty _) (λ x, .. (λ y, ι%T) ..))) 
+  (at level 200, x binder, y binder, right associativity,
+   format "'[ ' '∀S:' x .. y ,  κ  =>  ι  ']'") : sem_sig_scope.
+
+Notation "¡[ m ] σ" := (sem_sig_flip_mbang m σ) (at level 10) : sem_sig_scope.
+
+Notation "'∀S..:' tt , κ '=[' m ']=>' ι" := 
+  (sem_sig_flip_mbang m (sem_sig_eff (λ tt, κ%T) (λ tt, ι%T)))
+  (at level 200, tt binder, right associativity,
+   format "'[ ' '∀S..:' tt ,  κ  =[ m ]=>  ι  ']'") : sem_sig_scope.
+
+Notation "'∀S:' x .. y , κ '=[' m ']=>' ι" := 
+  (sem_sig_flip_mbang m (
+    (sem_sig_eff 
+    (@tele_app ((TeleS (λ x, .. (TeleS (λ y, TeleO)) ..))) (sem_ty _) (λ x, .. (λ y, κ%T) ..)) 
+    (@tele_app ((TeleS (λ x, .. (TeleS (λ y, TeleO)) ..))) (sem_ty _) (λ x, .. (λ y, ι%T) ..))))) 
+  (at level 200, x binder, y binder, right associativity,
+   format "'[ ' '∀S:' x .. y ,  κ  =[ m ]=>  ι  ']'") : sem_sig_scope.
+
+Lemma sem_sig_eff_mbang_eq {Σ} {TT : tele} A B m v Φ :
+  iEff_car (@sem_sig_flip_mbang Σ m (@sem_sig_eff Σ TT A B)) v Φ ⊣⊢
+    (∃.. αs, ∃ a, ⌜ a = v ⌝ ∗ (A αs a) ∗ 
+                            □? m (∀ b, (B αs b) -∗ Φ b))%I.
+Proof. 
+  rewrite /sem_sig_flip_mbang /=. 
+  iSplit.
+  - iIntros "(%Φ' & Hσ & HPost)". rewrite sem_sig_eff_eq.
+    iDestruct "Hσ" as "(%tt & % & %Heq & HA & HPost')".
+    iExists tt, a. iFrame. iSplit; first done. 
+    iDestruct (bi.intuitionistically_intuitionistically_if m with "HPost'") as "HPost'".
+    iDestruct (bi.intuitionistically_if_sep_2 with "[HPost HPost']") as "HPosts".
+    { by iSplitL "HPost". }
+    iApply (bi.intuitionistically_if_mono with "HPosts"). 
+    iIntros "[H1 H2] % HB". iApply "H1". by iApply "H2".
+  - iIntros "(%tt & % & %Heq & HA & HPost')".
+    iExists (λ b, B tt b). iFrame. rewrite sem_sig_eff_eq.
+    iExists tt, a. iFrame; iSplit; eauto.
+Qed.
+
+Section sig_properties.
+
 Global Instance sem_sig_eff_ne2 {Σ} {TT : tele} :
   NonExpansive2 (@sem_sig_eff Σ TT).
 Proof.
@@ -77,17 +138,6 @@ Proof.
   rewrite Hequiv. by apply sem_sig_eff_eq.
 Qed.
 
-(* Flip-Bang Signature *)
-Program Definition sem_sig_flip_mbang {Σ} (m : mode) (σ : sem_sig Σ) : sem_sig Σ := @PMonoProt Σ (upcl m σ) _.
-Next Obligation.
-  iIntros (??????) "#HΦ Hσ". 
-  destruct m.
-  - pose proof (upcl_mono_prot σ) as []. 
-    iApply (monotonic_prot with "HΦ Hσ").
-  - pose proof (pers_upcl_pers_mono_prot σ) as [].
-    iApply (pers_monotonic_prot with "HΦ Hσ").
-Qed.
-
 Global Instance sem_sig_flip_mbang_mono_prot {Σ} σ :
   MonoProt (@sem_sig_flip_mbang Σ OS σ).
 Proof. constructor. apply upcl_mono_prot. Qed.
@@ -105,140 +155,122 @@ Qed.
 Global Instance sem_sig_flip_mbang_proper {Σ} m : Proper ((≡) ==> (≡)) (@sem_sig_flip_mbang Σ m).
 Proof. apply ne_proper. apply _. Qed.
 
-(* Notations. *)
-Notation "'∀S..:' tt , κ '=>' ι" := 
-  (sem_sig_eff (λ tt, κ%T) (λ tt, ι%T))
-  (at level 200, tt binder, right associativity,
-   format "'[ ' '∀S..:' tt ,  κ  =>  ι  ']'") : sem_sig_scope.
+End sig_properties.
 
-Notation "'∀S:' x .. y , κ '=>' ι" := 
-  (sem_sig_eff 
-  (@tele_app ((TeleS (λ x, .. (TeleS (λ y, TeleO)) ..))) (sem_ty _) (λ x, .. (λ y, κ%T) ..)) 
-  (@tele_app ((TeleS (λ x, .. (TeleS (λ y, TeleO)) ..))) (sem_ty _) (λ x, .. (λ y, ι%T) ..))) 
-  (at level 200, x binder, y binder, right associativity,
-   format "'[ ' '∀S:' x .. y ,  κ  =>  ι  ']'") : sem_sig_scope.
+Section once_sig.
 
-Notation "¡_[ m ] σ" := (sem_sig_flip_mbang m σ) (at level 10) : sem_sig_scope.
+  (* Once Constraint *)
+  
+  Class OnceS {Σ} (σ : sem_sig Σ) := {
+    sig_le_mfbang_elim : (⊢ (¡[ OS ] σ) ≤ₛ σ)
+  }.
 
-Notation "'∀S..:' tt , κ '=[' m ']=>' ι" := 
-  (sem_sig_flip_mbang m (sem_sig_eff (λ tt, κ%T) (λ tt, ι%T)))
-  (at level 200, tt binder, right associativity,
-   format "'[ ' '∀S..:' tt ,  κ  =[ m ]=>  ι  ']'") : sem_sig_scope.
+End once_sig.
 
-Notation "'∀S:' x .. y , κ '=[' m ']=>' ι" := 
-  (sem_sig_flip_mbang m (
-    (sem_sig_eff 
-    (@tele_app ((TeleS (λ x, .. (TeleS (λ y, TeleO)) ..))) (sem_ty _) (λ x, .. (λ y, κ%T) ..)) 
-    (@tele_app ((TeleS (λ x, .. (TeleS (λ y, TeleO)) ..))) (sem_ty _) (λ x, .. (λ y, ι%T) ..))))) 
-  (at level 200, x binder, y binder, right associativity,
-   format "'[ ' '∀S:' x .. y ,  κ  =[ m ]=>  ι  ']'") : sem_sig_scope.
+Section sig_sub_typing.
 
-(* Subtyping on Signatures *)
+  (* Subtyping on Signatures *)
+  
+  Lemma sig_le_refl {Σ} (σ : sem_sig Σ) : ⊢ σ ≤ₛ σ.
+  Proof. iApply iEff_le_refl. Qed.
+  
+  Lemma sig_le_trans {Σ} (σ₁ σ₂ σ₃: sem_sig Σ) : 
+      σ₁ ≤ₛ σ₂ -∗
+      σ₂ ≤ₛ σ₃ -∗
+      σ₁ ≤ₛ σ₃. 
+  Proof. 
+    iIntros "#Hp₁₂ #Hp₂₃"; rewrite /sig_le /tc_opaque. 
+    iApply iEff_le_trans; [iApply "Hp₁₂"|iApply "Hp₂₃"].
+  Qed.
+  
+  Lemma sig_le_eff {Σ} {TT : tele} (ι₁ ι₂ κ₁ κ₂ : tele_arg TT → sem_ty Σ) :
+    □ (∀.. α, (ι₁ α) ≤ₜ (ι₂ α)) -∗
+    □ (∀.. α, (κ₂ α) ≤ₜ (κ₁ α)) -∗
+    (∀S..: α , ι₁ α => κ₁ α) ≤ₛ (∀S..: α , ι₂ α => κ₂ α).
+  Proof.
+    iIntros "#Hι₁₂ #Hκ₂₁". 
+    iIntros (v Φ) "!#".
+    rewrite !sem_sig_eff_eq.
+    iIntros "(%α & %w & <- & Hι₁ & HκΦ₁)".
+    iExists α, w; iSplitR; first done.
+    iSplitL "Hι₁".
+    { iApply ("Hι₁₂" with "Hι₁"). }
+    simpl. iDestruct "HκΦ₁" as "#HκΦ₁".
+    iIntros "!# %b Hκ₂". iApply "HκΦ₁".
+    iApply ("Hκ₂₁" with "Hκ₂").
+  Qed.
+  
+  Lemma sig_le_mfbang_intro {Σ} m (σ : sem_sig Σ) :
+    ⊢ σ ≤ₛ (¡[ m ] σ).
+  Proof.
+    rewrite /sem_sig_flip_mbang. 
+    iIntros (v Φ) "!# Hσ". simpl.
+    iExists Φ. iFrame. simpl. 
+    iApply bi.intuitionistically_intuitionistically_if.
+    iIntros "!# % $".
+  Qed.
+  
+  Lemma sig_le_mfbang_elim_ms {Σ} (σ : sem_sig Σ) :
+    ⊢ (¡[ MS ] σ) ≤ₛ σ.
+  Proof.
+    rewrite /sem_sig_flip_mbang. 
+    iIntros (v Φ) "!# (%Φ' & Hσ & HPost)". simpl.
+    by iApply (@pmono_prot_prop Σ σ with "HPost").
+  Qed.
+  
+  Lemma sig_le_mfbang_comp {Σ} (m m' : mode) (σ σ' : sem_sig Σ) :
+    m' ≤ₘ m -∗ σ ≤ₛ σ' -∗ 
+    (¡[ m ] σ) ≤ₛ (¡[ m' ] σ').
+  Proof.
+    iIntros "#Hlem #Hleσ". destruct m.
+    - iDestruct (mode_le_OS_inv with "Hlem") as "->".
+      rewrite /sig_le /sem_sig_flip_mbang /tc_opaque.
+      by iApply iEff_le_upcl.
+    - iApply sig_le_trans; first iApply sig_le_mfbang_elim_ms. 
+      iApply sig_le_trans; first iApply (sig_le_mfbang_intro m').
+      rewrite /sig_le /sem_sig_flip_mbang /tc_opaque.
+      by iApply iEff_le_upcl.
+  Qed.
+  
+  Lemma sig_le_mfbang_idemp {Σ} m (σ : sem_sig Σ) :
+    ⊢ (¡[ m ] (¡[ m ] σ)) ≤ₛ ((¡[ m ] σ)).
+  Proof. 
+    iIntros (v Φ) "!# (%Φ' & (%Φ'' & H & HPost') & HPost)". 
+    rewrite /sem_sig_flip_mbang /=.
+    iDestruct (bi.intuitionistically_if_sep_2 with "[HPost HPost']") as "HP"; first iFrame.
+    iExists Φ''. iFrame.
+    iApply (bi.intuitionistically_if_mono with "HP").
+    iIntros "[H1 H2] % HΦ''". iApply ("H2" with "[H1 HΦ'']"). 
+    by iApply "H1".
+  Qed.
 
-Lemma sig_le_refl {Σ} (σ : sem_sig Σ) : ⊢ σ ≤S σ.
-Proof. iApply iEff_le_refl. Qed.
+  Global Instance sig_fbang_once_sig {Σ} (σ : sem_sig Σ) : OnceS (¡[ OS ] σ)%S.
+  Proof. constructor. iIntros. iApply sig_le_mfbang_idemp. Qed.
 
-Lemma sig_le_trans {Σ} (σ₁ σ₂ σ₃: sem_sig Σ) : 
-    σ₁ ≤S σ₂ -∗
-    σ₂ ≤S σ₃ -∗
-    σ₁ ≤S σ₃. 
-Proof. 
-  iIntros "#Hp₁₂ #Hp₂₃"; rewrite /sig_le /tc_opaque. 
-  iApply iEff_le_trans; [iApply "Hp₁₂"|iApply "Hp₂₃"].
-Qed.
+  Global Instance sig_eff_os_once {TT : tele} {Σ} (A B : tele_arg TT → sem_ty Σ) :
+    OnceS (∀S..: αs , (A αs) =[ OS ]=> (B αs))%S.
+  Proof. apply _. Qed.
+  
+  Lemma sig_le_mfbang_comm {Σ} m m' (σ : sem_sig Σ) :
+    ⊢ (¡[ m ] (¡[ m' ] σ)) ≤ₛ (¡[ m' ] (¡[ m ] σ)).
+  Proof. 
+    destruct m, m'.
+    - iApply sig_le_refl.
+    - iApply sig_le_trans; first iApply sig_le_mfbang_comp.
+      { iApply mode_le_refl. }
+      { iApply sig_le_mfbang_elim_ms. }
+      iApply sig_le_mfbang_intro.
+    - iApply sig_le_trans; first iApply sig_le_mfbang_elim_ms.
+      iApply sig_le_mfbang_comp; first iApply mode_le_refl. 
+      iApply sig_le_mfbang_intro.
+    - iApply sig_le_refl.
+  Qed.
+  
+  Corollary sig_le_eff_mode {Σ} {TT : tele} (ι κ : tele_arg TT → sem_ty Σ) :
+    ⊢ (∀S..: α , ι α =[ MS ]=> κ α) ≤ₛ (∀S..: α , ι α =[ OS ]=> κ α).
+  Proof. 
+    iApply sig_le_mfbang_comp; first iApply mode_le_MS. 
+    iApply sig_le_refl. 
+  Qed.
 
-Lemma sig_le_eff {Σ} {TT : tele} (ι₁ ι₂ κ₁ κ₂ : tele_arg TT → sem_ty Σ) :
-  □ (∀.. α, (ι₁ α) ≤T (ι₂ α)) -∗
-  □ (∀.. α, (κ₂ α) ≤T (κ₁ α)) -∗
-  (∀S..: α , ι₁ α => κ₁ α) ≤S (∀S..: α , ι₂ α => κ₂ α).
-Proof.
-  iIntros "#Hι₁₂ #Hκ₂₁". 
-  iIntros (v Φ) "!#".
-  rewrite !sem_sig_eff_eq.
-  iIntros "(%α & %w & <- & Hι₁ & HκΦ₁)".
-  iExists α, w; iSplitR; first done.
-  iSplitL "Hι₁".
-  { iApply ("Hι₁₂" with "Hι₁"). }
-  simpl. iDestruct "HκΦ₁" as "#HκΦ₁".
-  iIntros "!# %b Hκ₂". iApply "HκΦ₁".
-  iApply ("Hκ₂₁" with "Hκ₂").
-Qed.
-
-Lemma sig_le_mfbang_intro {Σ} m (σ : sem_sig Σ) :
-  ⊢ σ ≤S (¡_[ m ] σ).
-Proof.
-  rewrite /sem_sig_flip_mbang. 
-  iIntros (v Φ) "!# Hσ". simpl.
-  iExists Φ. iFrame. simpl. 
-  iApply bi.intuitionistically_intuitionistically_if.
-  iIntros "!# % $".
-Qed.
-
-Lemma sig_le_mfbang_elim_ms {Σ} (σ : sem_sig Σ) :
-  ⊢ (¡_[ MS ] σ) ≤S σ.
-Proof.
-  rewrite /sem_sig_flip_mbang. 
-  iIntros (v Φ) "!# (%Φ' & Hσ & HPost)". simpl.
-  by iApply (@pmono_prot_prop Σ σ with "HPost").
-Qed.
-
-Lemma sig_le_mfbang_comp {Σ} (m m' : mode) (σ σ' : sem_sig Σ) :
-  m' ≤M m -∗ σ ≤S σ' -∗ 
-  (¡_[ m ] σ) ≤S (¡_[ m' ] σ').
-Proof.
-  iIntros "#Hlem #Hleσ". destruct m.
-  - iDestruct (mode_le_OS_inv with "Hlem") as "->".
-    rewrite /sig_le /sem_sig_flip_mbang /tc_opaque.
-    by iApply iEff_le_upcl.
-  - iApply sig_le_trans; first iApply sig_le_mfbang_elim_ms. 
-    iApply sig_le_trans; first iApply (sig_le_mfbang_intro m').
-    rewrite /sig_le /sem_sig_flip_mbang /tc_opaque.
-    by iApply iEff_le_upcl.
-Qed.
-
-Lemma sig_le_mfbang_idemp {Σ} m (σ : sem_sig Σ) :
-  ⊢ (¡_[ m ] (¡_[ m ] σ)) ≤S ((¡_[ m ] σ)).
-Proof. 
-  iIntros (v Φ) "!# (%Φ' & (%Φ'' & H & HPost') & HPost)". 
-  rewrite /sem_sig_flip_mbang /=.
-  iDestruct (bi.intuitionistically_if_sep_2 with "[HPost HPost']") as "HP"; first iFrame.
-  iExists Φ''. iFrame.
-  iApply (bi.intuitionistically_if_mono with "HP").
-  iIntros "[H1 H2] % HΦ''". iApply ("H2" with "[H1 HΦ'']"). 
-  by iApply "H1".
-Qed.
-
-Lemma sig_le_mfbang_comm {Σ} m m' (σ : sem_sig Σ) :
-  ⊢ (¡_[ m ] (¡_[ m' ] σ)) ≤S (¡_[ m' ] (¡_[ m ] σ)).
-Proof. 
-  destruct m, m'.
-  - iApply sig_le_refl.
-  - iApply sig_le_trans; first iApply sig_le_mfbang_comp.
-    { iApply mode_le_refl. }
-    { iApply sig_le_mfbang_elim_ms. }
-    iApply sig_le_mfbang_intro.
-  - iApply sig_le_trans; first iApply sig_le_mfbang_elim_ms.
-    iApply sig_le_mfbang_comp; first iApply mode_le_refl. 
-    iApply sig_le_mfbang_intro.
-  - iApply sig_le_refl.
-Qed.
-
-Corollary sig_le_eff_mode {Σ} {TT : tele} (ι κ : tele_arg TT → sem_ty Σ) :
-  ⊢ (∀S..: α , ι α =[ MS ]=> κ α) ≤S (∀S..: α , ι α =[ OS ]=> κ α).
-Proof. 
-  iApply sig_le_mfbang_comp; first iApply mode_le_MS. 
-  iApply sig_le_refl. 
-Qed.
-
-(* Once Constraint *)
-
-Class OnceS {Σ} (σ : sem_sig Σ) := {
-  flip_mbang_elim : (⊢ (¡_[ OS ] σ) ≤S σ)
-}.
-
-Global Instance sig_fbang_once_sig {Σ} (σ : sem_sig Σ) : OnceS (¡_[ OS ] σ)%S.
-Proof. constructor. iIntros. iApply sig_le_mfbang_idemp. Qed.
-
-Global Instance sig_eff_os_once {TT : tele} {Σ} (A B : tele_arg TT → sem_ty Σ) :
-  OnceS (∀S..: αs , (A αs) =[ OS ]=> (B αs))%S.
-Proof. apply _. Qed.
+End sig_sub_typing.
