theories/logic/sem_types.v
@@ -21,27 +21,23 @@ From affect.logic Require Import sem_def.
 From affect.logic Require Import mode.
 From affect.logic Require Import sem_sig.
 From affect.logic Require Import sem_row.
-From affect.logic Require Import sem_env.
 From affect.logic Require Import ewpw.
 
 (* Base types. *)
-Definition sem_ty_void {Σ} : sem_ty Σ := (λ v, False)%I.
+Definition sem_ty_bot {Σ} : sem_ty Σ := (λ v, False)%I.
+
+Global Instance sem_ty_bot_instance {Σ} : Bottom (sem_ty Σ) := sem_ty_bot. 
+
 Definition sem_ty_unit {Σ} : sem_ty Σ := (λ v, ⌜ v = #() ⌝)%I.
 Definition sem_ty_bool {Σ} : sem_ty Σ := (λ v, ∃ b : bool, ⌜ v = #b ⌝)%I.
 Definition sem_ty_int {Σ} : sem_ty Σ := (λ v, ∃ n : Z, ⌜ v = #n ⌝)%I.
 Definition sem_ty_string {Σ} : sem_ty Σ := (λ v, ∃ s : string, ⌜ v = #(LitStr s)⌝)%I.
 Definition sem_ty_top {Σ} : sem_ty Σ := (λ v, True)%I.
 
-Global Instance sem_ty_inhabited {Σ} : Inhabited (sem_ty Σ) := populate sem_ty_void. 
+Global Instance sem_ty_top_instance {Σ} : Top (sem_ty Σ) := sem_ty_top. 
+Global Instance sem_ty_inhabited {Σ} : Inhabited (sem_ty Σ) := populate sem_ty_top. 
 
-Definition sem_ty_bang {Σ} (τ : sem_ty Σ) : sem_ty Σ := (λ v, □ τ v)%I.
-(* generalised bang type *)
-Notation "'!_[ m ] τ" := (
-  match m with
-      OS => τ 
-    | MS => (sem_ty_bang τ)
-  end) (at level 10) : sem_ty_scope.
-Definition sem_env_bang {Σ} (Γ : env Σ) : env Σ := (map (λ xτ, (xτ.1, sem_ty_bang xτ.2)) Γ).
+Definition sem_ty_mbang {Σ} (m : mode) (τ : sem_ty Σ) : sem_ty Σ := (λ v, □? m (τ v))%I.
 
 (* Copyable Reference Type *)
 Definition tyN := nroot .@ "ty".
@@ -71,14 +67,14 @@ Definition sem_ty_arr `{heapGS Σ}
       EWPW (v w) <| ρ |> {{ u, κ u}})%I.
 
 (* Polymorphic type. *)
-Definition sem_ty_forall {Σ} 
+Definition sem_ty_type_forall {Σ} 
     (C : sem_ty Σ → sem_ty Σ) : sem_ty Σ := (λ v, ∀ τ, C τ v)%I.
 
 (* Polymorphic effect type. *)
 Definition sem_ty_row_forall {Σ} 
   (A : sem_row Σ → sem_ty Σ) : sem_ty Σ := (λ v, ∀ θ, A θ v)%I.
 
-(* Polymorphic type. *)
+(* Polymorphic mode type. *)
 Definition sem_ty_mode_forall {Σ} 
   (C : mode → sem_ty Σ) : sem_ty Σ := (λ v, ∀ ν, C ν v)%I.
 
@@ -110,18 +106,14 @@ Proof.
   - iIntros "HC //=". iNext. iExists (sem_ty_rec C).
     by iFrame. 
 Qed.
-Notation "'Void'" := sem_ty_void : sem_ty_scope.
-Notation "()" := sem_ty_unit : sem_ty_scope.
+
+Notation "'𝟙'" := sem_ty_unit : sem_ty_scope.
 Notation "'𝔹'" := (sem_ty_bool) : sem_ty_scope.
 Notation "'ℤ'" := (sem_ty_int) : sem_ty_scope.
 Notation "'Str'" := (sem_ty_string) : sem_ty_scope.
-Notation "⊤" := (sem_ty_top) : sem_ty_scope.
-Notation "'! τ " := (sem_ty_bang τ)
-  (at level 10) : sem_ty_scope.
-Notation "'! Γ " := (sem_env_bang Γ)
-  (at level 10) : sem_env_scope.
-Notation "τ '×' κ" := (sem_ty_prod τ%T κ%T)
-  (at level 120, κ at level 200) : sem_ty_scope.
+Notation "![ m ] τ" := (sem_ty_mbang m τ) (at level 10) : sem_ty_scope.
+
+Notation "τ '×' κ" := (sem_ty_prod τ%T κ%T) (at level 120) : sem_ty_scope.
 Infix "+" := (sem_ty_sum) : sem_ty_scope.
 
 Notation "'Ref' τ" := (sem_ty_ref τ%T) 
@@ -130,7 +122,7 @@ Notation "'Ref' τ" := (sem_ty_ref τ%T)
 Notation "'Refᶜ' τ" := (sem_ty_ref_cpy τ%T) 
   (at level 50) : sem_ty_scope.
 
-Notation "'∀T:' α , C " := (sem_ty_forall (λ α, C%T)) 
+Notation "'∀T:' α , C " := (sem_ty_type_forall (λ α, C%T)) 
   (at level 180) : sem_ty_scope.
 
 Notation "'∀R:' θ , C " := (sem_ty_row_forall (λ θ, C%T)) 
@@ -148,25 +140,23 @@ Notation "'μT:' α , C " := (sem_ty_rec (λ α, C%T))
 Notation "τ ⊸ κ" := (sem_ty_arr ⟨⟩%R τ%T κ%T)
   (at level 99, κ at level 200) : sem_ty_scope.
 
-Notation "τ '-{' ρ '}-[' m ']->' κ" := ('!_[ m ] (sem_ty_arr ρ%R τ%T κ%T))%T
-  (at level 100, m, ρ, κ at level 200) : sem_ty_scope.
-
-Notation "τ '-[' m ']->' κ" := ('!_[ m ] (sem_ty_arr ⟨⟩%R τ%T κ%T))%T
-  (at level 100, m, κ at level 200) : sem_ty_scope.
-
 Notation "τ '-{' ρ '}-∘' κ" := (sem_ty_arr ρ%R τ%T κ%T)
   (at level 100, ρ, κ at level 200) : sem_ty_scope.
-Notation "τ ⊸ κ" := (sem_ty_arr ⟨⟩%R τ%T κ%T)
-  (at level 99, κ at level 200) : sem_ty_scope.
 
-Notation "τ '-{' ρ '}->' κ" := (sem_ty_bang (sem_ty_arr ρ%R τ%T κ%T))
+Notation "τ '-{' ρ '}-[' m ']->' κ" := (sem_ty_mbang m (sem_ty_arr ρ%R τ%T κ%T))%T
+  (at level 100, m, ρ, κ at level 200) : sem_ty_scope.
+
+Notation "τ '-[' m ']->' κ" := (sem_ty_mbang m (sem_ty_arr ⟨⟩%R τ%T κ%T))%T
+  (at level 100, m, κ at level 200) : sem_ty_scope.
+
+Notation "τ '-{' ρ '}->' κ" := (sem_ty_mbang MS (sem_ty_arr ρ%R τ%T κ%T))
   (at level 100, ρ, κ at level 200) : sem_ty_scope.
-Notation "τ → κ" := (sem_ty_bang (sem_ty_arr ⟨⟩%R τ%T κ%T))
+
+Notation "τ → κ" := (sem_ty_mbang MS (sem_ty_arr ⟨⟩%R τ%T κ%T))
   (at level 99, κ at level 200) : sem_ty_scope.
 
 (* Derived Types *)
-
-Definition ListF {Σ} (τ : sem_ty Σ) := (λ α, () + (τ × α))%T.
+Definition ListF {Σ} (τ : sem_ty Σ) := (λ α, 𝟙 + (τ × α))%T.
 
 (* List type. *)
 Definition sem_ty_list {Σ} (τ : sem_ty Σ) : sem_ty Σ := 
@@ -176,7 +166,7 @@ Notation "'List' τ" := (sem_ty_list τ%T)
   (at level 50) : sem_ty_scope.
 
 (* List type. *)
-Definition sem_ty_option {Σ} (τ : sem_ty Σ) : sem_ty Σ := (() + τ)%T.
+Definition sem_ty_option {Σ} (τ : sem_ty Σ) : sem_ty Σ := (𝟙 + τ)%T.
 
 Notation "'Option' τ" := (sem_ty_option τ%T) 
   (at level 50) : sem_ty_scope.
@@ -189,13 +179,13 @@ Section types_properties.
 
   Ltac solve_non_expansive :=
     repeat intros ?;
-    unfold sem_ty_unit, sem_ty_int, sem_ty_bool, sem_ty_bang,
+    unfold sem_ty_unit, sem_ty_int, sem_ty_bool, sem_ty_mbang,
            sem_ty_prod, sem_ty_sum, sem_ty_arr,
            sem_ty_ref, sem_ty_ref_cpy, 
-           sem_ty_rec, sem_ty_list, sem_ty_forall, sem_ty_exists;
+           sem_ty_rec, sem_ty_list, sem_ty_type_forall, sem_ty_exists;
     repeat (f_equiv || done || intros ? || by apply non_dep_fun_dist).
 
-  Global Instance sem_ty_bang_ne : NonExpansive (@sem_ty_bang Σ).
+  Global Instance sem_ty_mbang_ne m : NonExpansive (@sem_ty_mbang Σ m).
   Proof. solve_non_expansive. Qed.
 
   Global Instance sem_ty_prod_ne : NonExpansive2 (@sem_ty_prod Σ).
@@ -213,21 +203,21 @@ Section types_properties.
   Global Instance sem_ty_ref_cpy_ne : NonExpansive (@sem_ty_ref_cpy Σ _).
   Proof. solve_non_expansive. Qed.
 
-  Global Instance sem_ty_forall_ne n :
-    Proper (pointwise_relation _ (dist n) ==> dist n) (@sem_ty_forall Σ).
+  Global Instance sem_ty_type_forall_ne n :
+    Proper (pointwise_relation _ (dist n) ==> dist n) (@sem_ty_type_forall Σ).
   Proof.
-    intros ????. unfold sem_ty_forall; repeat f_equiv. 
+    intros ????. unfold sem_ty_type_forall; repeat f_equiv. 
     by apply non_dep_fun_dist.
   Qed.
 
-  Global Instance sem_ty_forall_row_ne n :
+  Global Instance sem_ty_type_forall_row_ne n :
     Proper (pointwise_relation _ (dist n) ==> dist n) (@sem_ty_row_forall Σ).
   Proof.
     intros ????. unfold sem_ty_row_forall; repeat f_equiv.
     by apply non_dep_fun_dist.
   Qed.
 
-  Global Instance sem_ty_forall_mode_ne n :
+  Global Instance sem_ty_type_forall_mode_ne n :
     Proper (pointwise_relation _ (dist n) ==> dist n) (@sem_ty_mode_forall Σ).
   Proof.
     intros ????. unfold sem_ty_mode_forall; repeat f_equiv. 
@@ -263,7 +253,7 @@ Section types_properties.
          rewrite /ListF. intros ?. by repeat f_equiv.
   Qed.
 
-  Global Instance sem_ty_bang_proper : Proper ((≡) ==> (≡)) (@sem_ty_bang Σ).
+  Global Instance sem_ty_mbang_proper m : Proper ((≡) ==> (≡)) (@sem_ty_mbang Σ m).
   Proof. solve_non_expansive. Qed.
 
   Global Instance sem_ty_prod_proper : Proper ((≡) ==> (≡) ==> (≡)) (@sem_ty_prod Σ).
@@ -281,10 +271,10 @@ Section types_properties.
   Global Instance sem_ty_ref_cpy_proper : Proper ((≡) ==> (≡)) (@sem_ty_ref_cpy Σ _).
   Proof. intros ????. unfold sem_ty_ref_cpy; by repeat f_equiv. Qed.
 
-  Global Instance sem_ty_forall_proper :
-    Proper (pointwise_relation _ (≡) ==> (≡)) (@sem_ty_forall Σ).
+  Global Instance sem_ty_type_forall_proper :
+    Proper (pointwise_relation _ (≡) ==> (≡)) (@sem_ty_type_forall Σ).
   Proof. 
-    intros ????. unfold sem_ty_forall; repeat f_equiv. 
+    intros ????. unfold sem_ty_type_forall; repeat f_equiv. 
     by apply non_dep_fun_equiv. 
   Qed.
 
@@ -316,285 +306,78 @@ Section types_properties.
     apply sem_ty_rec_ne=> A. by apply equiv_dist.
   Qed.
 
-  Global Instance sem_ty_forall_type_persistent `{heapGS Σ} (C : sem_ty Σ → sem_ty Σ) v :
-    (∀ τ w, Persistent (C τ w)) →
-    Persistent ((sem_ty_forall C) v). 
-  Proof.
-    unfold sem_ty_forall. simpl. apply _.
-  Qed.
+  Global Instance sem_ty_mbang_persistent τ :
+    (∀ v, Persistent (@sem_ty_mbang Σ MS τ v)).
+  Proof. unfold sem_ty_mbang. simpl. apply _. Qed.
 
-  Global Instance sem_ty_row_forall_persistent `{heapGS Σ} (C : sem_row Σ → sem_ty Σ) v :
+  Global Instance sem_ty_type_forall_type_persistent (C : sem_ty Σ → sem_ty Σ) v :
+    (∀ τ w, Persistent (C τ w)) →
+    Persistent ((sem_ty_type_forall C) v). 
+  Proof. unfold sem_ty_type_forall. simpl. apply _. Qed.
+
+  Global Instance sem_ty_row_forall_persistent (C : sem_row Σ → sem_ty Σ) v :
     (∀ τ w, Persistent (C τ w)) →
     Persistent ((sem_ty_row_forall C) v).
-  Proof.
-    unfold sem_ty_row_forall. simpl. apply _.
-  Qed.
+  Proof. unfold sem_ty_row_forall. simpl. apply _. Qed.
 
-  Global Instance sem_ty_mode_forall_persistent `{heapGS Σ} (C : mode → sem_ty Σ) v :
+  Global Instance sem_ty_mode_forall_persistent (C : mode → sem_ty Σ) v :
     (∀ τ w, Persistent (C τ w)) →
     Persistent ((sem_ty_mode_forall C) v).
-  Proof.
-    unfold sem_ty_mode_forall. simpl. apply _.
-  Qed.
+  Proof. unfold sem_ty_mode_forall. simpl. apply _. Qed.
 
 End types_properties.
 
-Section copyable_types.
+Section multi_types.
   
   Context `{heapGS Σ}.
 
   Implicit Types τ κ : sem_ty Σ.
-
-  (* Copyable types *)
   
-  Open Scope sem_ty_scope.
+  Class MultiT {Σ} (τ : sem_ty Σ) := {
+    multi_ty : ⊢ (τ%T ≤ₜ ![ MS ] τ%T)
+  }.
 
-  Lemma copy_ty_void : ⊢ @copy_ty Σ Void.
-  Proof. iIntros "!# %v $!". Qed.
+  Global Arguments MultiT _ _%T.
 
-  Lemma copy_ty_unit : ⊢ @copy_ty Σ ().
-  Proof. iIntros "!# %v $!". Qed.
-  
-  Lemma copy_ty_bool : ⊢ @copy_ty Σ 𝔹.
-  Proof. iIntros "!# %v #$". Qed.
-  
-  Lemma copy_ty_nat : ⊢ @copy_ty Σ ℤ.
-  Proof. iIntros "!# %v #$". Qed.
-  
-  Lemma copy_ty_top : ⊢ @copy_ty Σ ⊤.
-  Proof. iIntros "!# %v #$". Qed.
-
-  Lemma copy_ty_bang τ : ⊢ copy_ty ('! τ).
-  Proof. iIntros "!# %v #$". Qed.
-
-  Lemma copy_ty_uarr τ σ κ : ⊢ copy_ty (τ -{ σ }-> κ).
-  Proof. apply copy_ty_bang. Qed.
-  
-  Lemma copy_ty_prod τ κ : copy_ty τ -∗ copy_ty κ -∗ copy_ty (τ × κ).
+  Global Instance multi_ty_persistent (τ : sem_ty Σ) `{! MultiT τ} :
+    ∀ v, Persistent (τ v).
   Proof. 
-    iIntros "#Hcpyτ #Hcpyκ !# %v (% & % & -> & Hτ & Hκ)". 
-    iDestruct ("Hcpyτ" with "Hτ") as "#Hτ'".
-    iDestruct ("Hcpyκ" with "Hκ") as "#Hκ'". 
-    iIntros "!#". iExists v₁, v₂. by iFrame "#".
+    intros ?. inv MultiT0. 
+    rewrite /ty_le /tc_opaque /sem_ty_mbang /= in multi_ty0.
+    rewrite /Persistent. 
+    iIntros "Hτ.". iDestruct (multi_ty0 with "Hτ.") as "#Hτ".
+    by iModIntro.
   Qed.
 
-  Lemma copy_ty_sum τ κ : copy_ty τ -∗ copy_ty κ -∗ copy_ty (τ + κ).
-  Proof.
-    iIntros "#Hcpyτ #Hcpyκ !# %v (% & [(-> & Hτ)|(-> & Hκ)])". 
-    - iDestruct ("Hcpyτ" with "Hτ") as "#Hτ'". iIntros "!#". 
-      iExists v'. iLeft. by iFrame "#".
-    - iDestruct ("Hcpyκ" with "Hκ") as "#Hκ'". iIntros "!#". 
-      iExists v'. iRight. by iFrame "#".
-  Qed.
-
-  Lemma copy_ty_forallT (C : _ → sem_ty Σ) :
-    (∀ α, copy_ty (C α)) -∗ copy_ty (∀T: α, C α).
-  Proof. iIntros "#H !# % HC /= %T". by iApply "H". Qed.
-
-  Lemma copy_ty_forallR (C : _ → sem_ty Σ) :
-    (∀ θ, copy_ty (C θ)) -∗ copy_ty (∀R: θ, C θ).
-  Proof. iIntros "#H !# % HC /= %T". by iApply "H". Qed.
-
-  Lemma copy_ty_forallM (C : _ → sem_ty Σ) :
-    (∀ ν, copy_ty (C ν)) -∗ copy_ty (∀M: ν, C ν).
-  Proof. iIntros "#H !# % HC /= %T". by iApply "H". Qed.
-
-  Lemma copy_ty_ref τ : ⊢ copy_ty (Refᶜ τ).
-  Proof. iIntros "!# % #$". Qed.
-
-  Lemma copy_ty_exists A : (∀ α, copy_ty (A α)) -∗ copy_ty (∃: α, A α).
-  Proof. 
-    iIntros "#H !# % [%α Hτ']". 
-    iDestruct ("H" with "Hτ'") as "#Hτ".
-    iIntros "!#". by iExists α.
-  Qed.
-
-  Lemma copy_ty_rec A `{NonExpansive A}: 
-    □ (∀ α, (copy_ty α) -∗ copy_ty (A α)) -∗ 
-    @copy_ty Σ (μT: α, A α).
-  Proof. 
-    iIntros "#H !# %". iLöb as "IH" forall (v). 
-    rewrite {1 2} sem_ty_rec_unfold.
-    iIntros "Hτ". iApply bi.later_intuitionistically.
-    iNext. iApply ("H" with "[] Hτ"). 
-    rewrite /copy_ty /tc_opaque. iApply "IH".
-  Qed.
-
-  Lemma copy_ty_option τ : copy_ty τ -∗ copy_ty (Option τ).
-  Proof. 
-    iIntros "#H". 
-    iApply copy_ty_sum; [iApply copy_ty_unit|done]. 
-  Qed.
-
-  Lemma copy_ty_list τ : copy_ty τ -∗ copy_ty (List τ).
-  Proof.
-    iIntros "#Hτ". iApply copy_ty_rec.
-    iIntros "!# % #Hα". 
-    iApply copy_ty_sum; [iApply copy_ty_unit|].
-    by iApply copy_ty_prod.
-  Qed.
-
-  Lemma copy_env_nil : ⊢ @copy_env Σ [].
-  Proof. iIntros "!# % #$". Qed.
-  
-  Lemma copy_env_cons Γ x τ : 
-    copy_env Γ -∗
-    copy_ty τ -∗
-    copy_env ((x, τ) :: Γ).
-  Proof. 
-    iIntros "#HΓcpy #Hτcpy !# % (% & %Hrw & Hτ & HΓ)".
-    iDestruct ("Hτcpy" with "Hτ") as "#Hτ'".
-    iDestruct ("HΓcpy" with "HΓ") as "#HΓ'".
-    iIntros "!#". iExists v. by iFrame "#".
-  Qed.
-
-End copyable_types.
-
-Section type_sub.
-
-(* Subsumption relation on modes and rows wrt to types *)
-
-Lemma row_type_sub_copy {Σ} (ρ : sem_row Σ) (τ : sem_ty Σ) : copy_ty τ -∗ ρ ≼ₜ τ.
-Proof.
-  iIntros "#Hτcpy %w %v %Φ !# Hρ Hτ.".
-  iDestruct ("Hτcpy" with "Hτ.") as "#Hτ".
-  iApply (pmono_prot_prop _ (sem_row_car ρ) with "[] Hρ").
-  iIntros "!# % H". iFrame "#". iApply "H".
-Qed.
-
-Lemma row_type_sub_bang {Σ} (ρ : sem_row Σ) (τ : sem_ty Σ) : ⊢ ρ ≼ₜ ('! τ).
-Proof.
-  iIntros (w v Φ) "!# Hρ #Hτ".
-  iApply (pmono_prot_prop _ (sem_row_car ρ) with "[] Hρ").
-  iIntros "!# % $ //".
-Qed.
-
-Lemma row_type_sub_mfbang_mbang {Σ} (m : mode) (ρ : sem_row Σ) (τ : sem_ty Σ) : ⊢ ¡_[ m ] ρ ≼ₜ ('!_[ m ] τ).
-Proof. destruct m; [iApply row_type_sub_fbang|iApply row_type_sub_bang]. Qed.
-
-Lemma mode_type_sub_mbang {Σ} m (τ : sem_ty Σ) : ⊢ m ₘ≼ₜ '!_[m] τ.
-Proof. 
-  rewrite /mode_type_sub /=. iIntros "!# % Hτ". 
-  destruct m; simpl; first done. iApply "Hτ".
-Qed.
-
-Lemma mode_type_sub_mbang_meet {Σ} (m m' : mode) (τ : sem_ty Σ) : ⊢ m ⊓ₘ m' ₘ≼ₜ ('!_[ m ] τ).
-Proof. 
-  destruct m; first rewrite mode_glb_os; first iApply mode_type_sub_os.
-  iApply mode_type_sub_ms. iApply copy_ty_bang.
-Qed.
-
-End type_sub.
+End multi_types.
 
 Section sub_typing.
 
   Context `{!heapGS Σ}.
 
-  Lemma ty_le_refl (τ : sem_ty Σ) : ⊢ τ ≤T τ.
+  Implicit Types τ κ : sem_ty Σ.
+
+  Lemma ty_le_refl (τ : sem_ty Σ) : ⊢ τ ≤ₜ τ.
   Proof. iIntros "!# % $". Qed.
 
   Lemma ty_le_trans (τ₁ τ₂ τ₃ : sem_ty Σ) :
-    τ₁ ≤T τ₂ -∗
-    τ₂ ≤T τ₃ -∗
-    τ₁ ≤T τ₃.
+    τ₁ ≤ₜ τ₂ -∗
+    τ₂ ≤ₜ τ₃ -∗
+    τ₁ ≤ₜ τ₃.
   Proof. 
     iIntros "#Hτ₁₂ #Hτ₂₃ !# %v Hτ₁". 
     iApply "Hτ₂₃". by iApply "Hτ₁₂".
   Qed.
 
-  Lemma ty_le_void (τ : sem_ty Σ) :
-    ⊢ Void ≤T τ.
+  Lemma ty_le_bot (τ : sem_ty Σ) :
+    ⊢ ⊥ ≤ₜ τ.
   Proof. iIntros "% !# []". Qed.
 
-  Lemma ty_le_mbang_intro m (τ : sem_ty Σ) :
-    copy_ty τ -∗
-    τ ≤T '!_[m] τ.
-  Proof. 
-    iIntros "#Hcpy".
-    destruct m; simpl; first iApply ty_le_refl.
-    iIntros "!# %v Hτ". 
-    iDestruct ("Hcpy" with "Hτ") as "#Hτ'".
-    iIntros "!# {$#Hτ'}". 
-  Qed.
-
-  Lemma ty_le_bang_elim (τ : sem_ty Σ) :
-    ⊢ ('! τ) ≤T τ.
-  Proof. iIntros "!# %v #$". Qed.
-
-
-  Lemma ty_le_mbang_elim (m : mode) (τ : sem_ty Σ) :
-    ⊢ ('!_[m] τ) ≤T τ.
-  Proof. destruct m; first iApply ty_le_refl. iApply ty_le_bang_elim. Qed.
-
-  Lemma ty_le_bang_comp (τ1 τ2 : sem_ty Σ) :
-    τ1 ≤T τ2 -∗ ('! τ1) ≤T ('! τ2).
-  Proof. iIntros "#Hττ' !# %v #H!τ !#". by iApply "Hττ'". Qed.
-
-  Lemma ty_le_mbang_comp m (τ τ' : sem_ty Σ) :
-    τ ≤T τ' -∗ ('!_[m] τ) ≤T ('!_[m] τ').
-  Proof. iIntros "#Hττ'". destruct m; [done|by iApply ty_le_bang_comp]. Qed.
-
-  Lemma ty_le_mbang_idemp m (τ : sem_ty Σ) :
-    ⊢ '!_[m] τ ≤T '!_[m] ('!_[m] τ).
-  Proof. 
-    destruct m; simpl; first iApply ty_le_refl.
-    iApply (ty_le_mbang_intro MS). iApply copy_ty_bang.
-  Qed.
-
-  Lemma ty_le_mbang_idemp_inv m (τ : sem_ty Σ) :
-    ⊢ '!_[m] ('!_[m] τ) ≤T '!_[m] τ.
-  Proof. 
-    destruct m; simpl; first iApply ty_le_refl.
-    iApply (ty_le_mbang_elim MS).
-  Qed.
-
-  Lemma ty_le_mbang_comm m m' (τ : sem_ty Σ) :
-    ⊢ '!_[m] ('!_[m'] τ) ≤T '!_[m'] ('!_[m] τ). 
-  Proof. 
-    destruct m, m'; iApply ty_le_refl.
-  Qed.
-
-  Lemma ty_le_mbang_mode_le m m' (τ : sem_ty Σ) :
-    ⊢ m' ≤M m -∗ ('!_[m] τ) ≤T ('!_[m'] τ). 
-  Proof. 
-    iIntros "H". destruct m.
-    - iDestruct (mode_le_OS_inv with "H") as "->".
-      iApply ty_le_refl.
-    - destruct m'; [iApply (ty_le_mbang_elim MS)|iApply ty_le_refl].
-  Qed.
-
   Lemma ty_le_arr (τ₁ κ₁ τ₂ κ₂ : sem_ty Σ) (ρ ρ' : sem_row Σ) :
-    ρ ≤R ρ' -∗
-    τ₂ ≤T τ₁ -∗
-    κ₁ ≤T κ₂ -∗
-    (τ₁ -{ ρ }-∘ κ₁) ≤T (τ₂ -{ ρ' }-∘ κ₂).
-  Proof.
-    iIntros "#Hρ  #Hτ₂₁ #Hκ₁₂ !# %v Hτκ₁". 
-    rewrite /sem_ty_arr /=. iIntros "% Hτ₂".
-    iApply (ewpw_sub with "Hρ").
-    iApply (ewpw_mono with "[Hτκ₁ Hτ₂]").
-    { iApply ("Hτκ₁" with "[Hτ₂]"); by iApply "Hτ₂₁". }
-    iIntros "!# % Hκ !>". by iApply "Hκ₁₂".
-  Qed.
-
-  Lemma ty_le_uarr (τ₁ κ₁ τ₂ κ₂ : sem_ty Σ) (ρ ρ' : sem_row Σ) :
-    ρ ≤R ρ' -∗
-    τ₂ ≤T τ₁ -∗
-    κ₁ ≤T κ₂ -∗
-    (τ₁ -{ ρ }-> κ₁) ≤T (τ₂ -{ ρ' }-> κ₂).
-  Proof.
-    iIntros "#Hρ  #Hτ₂₁ #Hκ₁₂". iApply ty_le_bang_comp. by iApply ty_le_arr.
-  Qed.
-      
-  Lemma ty_le_u2aarr (τ κ : sem_ty Σ) (ρ : sem_row Σ) :
-    ⊢ (τ -{ ρ }-> κ) ≤T (τ -{ ρ }-∘ κ).
-  Proof. apply ty_le_bang_elim. Qed.
-
-  Lemma ty_le_aarr (τ₁ κ₁ τ₂ κ₂ : sem_ty Σ) (ρ ρ' : sem_row Σ) :
-    ρ ≤R ρ' -∗
-    τ₂ ≤T τ₁ -∗
-    κ₁ ≤T κ₂ -∗
-    (τ₁ -{ ρ }-∘ κ₁) ≤T (τ₂ -{ ρ' }-∘ κ₂).
+    ρ ≤ᵣ ρ' -∗
+    τ₂ ≤ₜ τ₁ -∗
+    κ₁ ≤ₜ κ₂ -∗
+    (τ₁ -{ ρ }-∘ κ₁) ≤ₜ (τ₂ -{ ρ' }-∘ κ₂).
   Proof.
     iIntros "#Hρ  #Hτ₂₁ #Hκ₁₂ !# %v Hτκ₁". 
     rewrite /sem_ty_arr /=. iIntros "% Hτ₂".
@@ -605,8 +388,8 @@ Section sub_typing.
   Qed.
 
   Lemma ty_le_ref (τ₁ τ₂ : sem_ty Σ) :
-    τ₁ ≤T τ₂ -∗
-    (Ref τ₁) ≤T (Ref τ₂).
+    τ₁ ≤ₜ τ₂ -∗
+    (Ref τ₁) ≤ₜ (Ref τ₂).
   Proof.
     iIntros "#Hτ₁₂ !# %v (%l & -> & (%w & Hl & Hτw))".
     iExists l. iSplit; first done.
@@ -614,9 +397,9 @@ Section sub_typing.
   Qed.
 
   Lemma ty_le_prod (τ₁ τ₂ κ₁ κ₂ : sem_ty Σ) :
-    τ₁ ≤T τ₂ -∗
-    κ₁ ≤T κ₂ -∗
-    (τ₁ × κ₁) ≤T (τ₂ × κ₂).
+    τ₁ ≤ₜ τ₂ -∗
+    κ₁ ≤ₜ κ₂ -∗
+    (τ₁ × κ₁) ≤ₜ (τ₂ × κ₂).
   Proof.
     iIntros "#Hτ₁₂ #Hκ₁₂ !# %v (%w₁ & %w₂ & -> &Hw₁ & Hw₂)".
     iExists w₁, w₂. iSplit; first done. iSplitL "Hw₁".
@@ -624,91 +407,47 @@ Section sub_typing.
     by iApply "Hκ₁₂".
   Qed.
   
-  Lemma ty_le_mbang_prod_intro m (τ κ : sem_ty Σ) :
-    τ ≤T '!_[m] τ -∗
-    κ ≤T '!_[m] κ -∗
-    (τ × κ) ≤T '!_[m] (τ × κ).
-  Proof.
-    iIntros "#Hτ #Hκ". 
-    destruct m; simpl; first iApply ty_le_refl.
-    iApply (ty_le_mbang_intro MS).
-    iApply (copy_ty_prod with "Hτ Hκ").
-  Qed.
-
   Lemma ty_le_sum (τ₁ τ₂ κ₁ κ₂ : sem_ty Σ) :
-    τ₁ ≤T τ₂ -∗
-    κ₁ ≤T κ₂ -∗
-    (τ₁ + κ₁) ≤T (τ₂ + κ₂).
+    τ₁ ≤ₜ τ₂ -∗
+    κ₁ ≤ₜ κ₂ -∗
+    (τ₁ + κ₁) ≤ₜ (τ₂ + κ₂).
   Proof.
     iIntros "#Hτ₁₂ #Hκ₁₂ !# %v (%v' & [(-> & Hτ₁)|(-> & Hκ₁)])"; iExists v'. 
     - iLeft. iSplit; first done. by iApply "Hτ₁₂".
     - iRight. iSplit; first done. by iApply "Hκ₁₂". 
   Qed.
 
-  Lemma ty_le_mbang_sum_intro m (τ κ : sem_ty Σ) :
-    τ ≤T '!_[m] τ -∗
-    κ ≤T '!_[m] κ -∗
-    (τ + κ) ≤T '!_[m] (τ + κ).
-  Proof.
-    iIntros "#Hτ #Hκ". 
-    destruct m; simpl; first iApply ty_le_refl.
-    iApply (ty_le_mbang_intro MS).
-    iApply (copy_ty_sum with "Hτ Hκ").
-  Qed.
-
-  Lemma ty_le_option (τ₁ τ₂ : sem_ty Σ) :
-    τ₁ ≤T τ₂ -∗
-    (Option τ₁) ≤T (Option τ₂).
+  Corollary ty_le_option (τ₁ τ₂ : sem_ty Σ) :
+    τ₁ ≤ₜ τ₂ -∗
+    (Option τ₁) ≤ₜ (Option τ₂).
   Proof. iIntros "#?". iApply ty_le_sum; last done. iIntros "!# % $". Qed.
 
-  Lemma ty_le_forall (τ₁ τ₂ : sem_ty Σ → sem_ty Σ) :
-    (∀ α, τ₁ α ≤T τ₂ α) -∗
-    (∀T: α, τ₁ α)%T ≤T (∀T: α, τ₂ α).
+  Lemma ty_le_type_forall (τ₁ τ₂ : sem_ty Σ → sem_ty Σ) :
+    (∀ α, τ₁ α ≤ₜ τ₂ α) -∗
+    (∀T: α, τ₁ α)%T ≤ₜ (∀T: α, τ₂ α).
   Proof. iIntros "#Hτ₁₂ !# %v Hτ₁ %τ /=". by iApply "Hτ₁₂". Qed.
-
-  Lemma ty_le_bang_forall (τ : sem_ty Σ → sem_ty Σ) :
-    ⊢ (∀T: α, '! (τ α))%T ≤T '! (∀T: α, τ α).
-  Proof. iIntros "!# %v #Hτ !> %σ". iApply "Hτ". Qed.
-
-  Lemma ty_le_forall_bang (τ : sem_ty Σ → sem_ty Σ) :
-    ⊢ '! (∀T: α, τ α) ≤T (∀T: α, '! (τ α))%T.
-  Proof. iIntros "!# %v #Hτ %σ !>". iApply "Hτ". Qed.
 
   Lemma ty_le_row_forall (τ₁ τ₂ : sem_row Σ → sem_ty Σ) :
-    (∀ θ, τ₁ θ ≤T τ₂ θ) -∗
-    (∀R: θ, τ₁ θ) ≤T (∀R: θ, τ₂ θ).
+    (∀ θ, τ₁ θ ≤ₜ τ₂ θ) -∗
+    (∀R: θ, τ₁ θ) ≤ₜ (∀R: θ, τ₂ θ).
   Proof. iIntros "#Hτ₁₂ !# %v Hτ₁ %τ /=". by iApply "Hτ₁₂". Qed.
-
-  Lemma ty_le_bang_row_forall (τ : sem_row Σ → sem_ty Σ) :
-    ⊢ (∀R: θ, '! (τ θ))%T ≤T '! (∀R: θ, τ θ).
-  Proof. iIntros "!# %v #Hτ !> %θ". iApply "Hτ". Qed.
-  Lemma ty_le_row_forall_bang (τ : sem_row Σ → sem_ty Σ) :
-    ⊢ '! (∀R: θ, τ θ) ≤T (∀R: θ, '! (τ θ))%T.
-  Proof. iIntros "!# %v #Hτ %θ !>". iApply "Hτ". Qed.
 
   Lemma ty_le_mode_forall (τ₁ τ₂ : mode → sem_ty Σ) :
-    (∀ ν, τ₁ ν ≤T τ₂ ν) -∗
-    (∀M: ν, τ₁ ν) ≤T (∀M: ν, τ₂ ν).
+    (∀ ν, τ₁ ν ≤ₜ τ₂ ν) -∗
+    (∀M: ν, τ₁ ν) ≤ₜ (∀M: ν, τ₂ ν).
   Proof. iIntros "#Hτ₁₂ !# %v Hτ₁ %τ /=". by iApply "Hτ₁₂". Qed.
 
-  Lemma ty_le_bang_mode_forall (τ : mode → sem_ty Σ) :
-    ⊢ (∀M: ν, '! (τ ν))%T ≤T '! (∀M: ν, τ ν).
-  Proof. iIntros "!# %v #Hτ !> %ν". iApply "Hτ". Qed.
-  Lemma ty_le_mode_forall_bang (τ : mode → sem_ty Σ) :
-    ⊢ '! (∀M: ν, τ ν) ≤T (∀M: ν, '! (τ ν))%T.
-  Proof. iIntros "!# %v #Hτ %ν !>". iApply "Hτ". Qed.
-
   Lemma ty_le_exists (τ₁ τ₂ : sem_ty Σ → sem_ty Σ) :
-    (∀ α, τ₁ α ≤T τ₂ α) -∗
-    (∃: α, τ₁ α) ≤T (∃: α, τ₂ α).
+    (∀ α, τ₁ α ≤ₜ τ₂ α) -∗
+    (∃: α, τ₁ α) ≤ₜ (∃: α, τ₂ α).
   Proof.
     iIntros "#Hτ₁₂ !# %v (%α & Hα) //=".
     iExists α. by iApply "Hτ₁₂".
   Qed.
 
   Lemma ty_le_rec (τ₁ τ₂ : sem_ty Σ -> sem_ty Σ) `{NonExpansive τ₁, NonExpansive τ₂} :
-    □ (∀ α α', (α ≤T α') -∗ τ₁ α ≤T τ₂ α') -∗
-    (μT: α, τ₁ α) ≤T (μT: α, τ₂ α).
+    □ (∀ α α', (α ≤ₜ α') -∗ τ₁ α ≤ₜ τ₂ α') -∗
+    (μT: α, τ₁ α) ≤ₜ (μT: α, τ₂ α).
   Proof.
     iIntros "#Hτ₁₂ !#". iLöb as "IH". iIntros "%v Hτ₁".
     iApply sem_ty_rec_unfold.
@@ -717,48 +456,358 @@ Section sub_typing.
     rewrite /ty_le /tc_opaque. iApply "IH".
   Qed.
   
-  Lemma ty_le_rec_bang m (τ : sem_ty Σ -> sem_ty Σ) `{NonExpansive τ} :
-    □ (∀ α, (α ≤T '!_[m] α) -∗ τ α ≤T '!_[m] (τ α)) -∗
-    (μT: α, τ α) ≤T '!_[m] (μT: α, τ α).
+  Corollary ty_le_list (τ₁ τ₂ : sem_ty Σ) :
+    τ₁ ≤ₜ τ₂ -∗
+    List τ₁ ≤ₜ List τ₂.
+  Proof.
+    rewrite /sem_ty_list. iIntros "#Hτ₁₂".
+    iApply ty_le_rec. iIntros "!# % % Hαα'".
+    iApply ty_le_sum; first iApply ty_le_refl.
+    by iApply ty_le_prod.
+  Qed.
+
+  Lemma ty_le_mbang_intro_os τ : ⊢ τ ≤ₜ ![OS] τ.
+  Proof. iIntros "!# %v H". rewrite /sem_ty_mbang //. Qed.
+
+  Corollary ty_le_mbang_intro_void m τ : ⊢ ⊥ ≤ₜ ![m] τ.
+  Proof. iApply ty_le_bot. Qed.
+
+  Global Instance multi_ty_void : @MultiT Σ ⊥.
+  Proof. constructor. iApply ty_le_mbang_intro_void. Qed.
+
+  Lemma ty_le_mbang_intro_unit m : ⊢ 𝟙 ≤ₜ@{ Σ } ![m] 𝟙.
+  Proof. 
+    iIntros "!# %v ->". 
+    iApply bi.intuitionistically_intuitionistically_if. 
+    iIntros "!# //".
+  Qed.
+
+  Global Instance multi_ty_unit : @MultiT Σ 𝟙.
+  Proof. constructor. iApply ty_le_mbang_intro_unit. Qed.
+  
+  Lemma ty_le_mbang_intro_bool m : ⊢ 𝔹 ≤ₜ@{ Σ } ![m] 𝔹.
+  Proof. 
+    iIntros "!# %v (% & ->)". 
+    iApply bi.intuitionistically_intuitionistically_if. 
+    iIntros "!#". by iExists b.
+  Qed.
+
+  Global Instance multi_ty_bool : @MultiT Σ 𝔹.
+  Proof. constructor. iApply ty_le_mbang_intro_bool. Qed.
+
+  Lemma ty_le_mbang_intro_int m : ⊢ ℤ ≤ₜ@{ Σ } ![m] ℤ.
+    iIntros "!# %v (% & ->)". 
+    iApply bi.intuitionistically_intuitionistically_if. 
+    iIntros "!#". by iExists n.
+  Qed.
+
+  Global Instance multi_ty_int : @MultiT Σ ℤ.
+  Proof. constructor. iApply ty_le_mbang_intro_int. Qed.
+  
+  Lemma ty_le_mbang_intro_top m : ⊢ ⊤ ≤ₜ@{ Σ } ![m] ⊤.
+  Proof. 
+    iIntros "!# %v _". 
+    iApply bi.intuitionistically_intuitionistically_if. 
+    by iIntros "!#".
+  Qed.
+
+  Global Instance multi_ty_top : @MultiT Σ ⊤.
+  Proof. constructor. iApply ty_le_mbang_intro_top. Qed.
+
+  Lemma ty_le_mbang_idemp m τ : ⊢ (![m] τ ≤ₜ ![m] (![m] τ)).
+  Proof. 
+    iIntros "!# %v H".
+    iApply bi.intuitionistically_if_idemp. 
+    iApply "H".
+  Qed.
+
+  Global Instance multi_ty_mbang τ : MultiT (![MS] τ).
+  Proof. constructor. iApply ty_le_mbang_idemp. Qed.
+
+  Corollary ty_le_mbang_intro_uarr τ ρ κ : ⊢ (τ -{ ρ }-> κ) ≤ₜ (![MS] (τ -{ ρ }-> κ)).
+  Proof. iApply ty_le_mbang_idemp. Qed.
+
+  Corollary multi_ty_uarr τ ρ κ : MultiT (τ -{ ρ }-> κ).
+  Proof. apply _. Qed.
+
+  Lemma ty_le_mbang_intro_prod τ κ m : τ ≤ₜ ![m] τ -∗ κ ≤ₜ ![m] κ -∗ (τ × κ) ≤ₜ ![m] (τ × κ).
+  Proof. 
+    iIntros "#Hτle #Hκle !# %v (% & % & -> & Hτ & Hκ)". 
+    iDestruct ("Hτle" with "Hτ") as "Hτ".
+    iDestruct ("Hκle" with "Hκ") as "Hκ". 
+    iDestruct (bi.intuitionistically_if_sep_2 with "[Hτ Hκ]") as "H"; first iFrame.
+    iApply (bi.intuitionistically_if_mono with "H").
+    iIntros "[Hκ Hτ]". iExists v₁, v₂. by iFrame.
+  Qed.
+
+  Global Instance multi_ty_prod τ κ `{!MultiT τ} `{!MultiT κ} : MultiT (τ × κ).
+  Proof. constructor. inv MultiT0. inv MultiT1. by iApply ty_le_mbang_intro_prod. Qed.
+
+  Lemma ty_le_mbang_intro_sum τ κ m : τ ≤ₜ ![m] τ -∗ κ ≤ₜ ![m] κ -∗ (τ + κ) ≤ₜ ![m] (τ + κ).
+  Proof.
+    iIntros "#Hτle #Hκle !# %v (% & [(-> & Hτ)|(-> & Hκ)])". 
+    - iDestruct ("Hτle" with "Hτ") as "Hτ". 
+      iApply (bi.intuitionistically_if_mono with "Hτ").
+      iIntros "Hτ". iExists v'. iLeft. by iFrame.
+    - iDestruct ("Hκle" with "Hκ") as "Hκ".
+      iApply (bi.intuitionistically_if_mono with "Hκ").
+      iIntros "Hκ". iExists v'. iRight. by iFrame.
+  Qed.
+
+  Global Instance multi_ty_sum τ κ `{!MultiT τ} `{!MultiT κ} : MultiT (τ + κ).
+  Proof. constructor. inv MultiT0. inv MultiT1. by iApply ty_le_mbang_intro_sum. Qed.
+
+  Lemma ty_le_mbang_intro_type_forall (C : sem_ty Σ → sem_ty Σ) m :
+    (∀ α, (C α) ≤ₜ ![m] (C α)) -∗ (∀T: α, C α) ≤ₜ ![m] (∀T: α, C α).
+  Proof. 
+    iIntros "#Hle % !# H". rewrite /sem_ty_mbang /sem_ty_type_forall.
+    iApply forall_intuitionistically_if. iIntros (τ).
+    iApply ("Hle" with "H").
+  Qed.
+
+  Global Instance multi_ty_type_forall (C : sem_ty Σ → sem_ty Σ) `{! ∀ α, MultiT (C α) } : 
+    MultiT (∀T: α, C α).
+  Proof. 
+    constructor. iApply ty_le_mbang_intro_type_forall. 
+    iIntros (τ). specialize (H τ). inv H. iApply multi_ty0.
+  Qed.
+
+  Lemma ty_le_mbang_intro_row_forall (C : sem_row Σ → sem_ty Σ) m :
+    (∀ θ, (C θ) ≤ₜ ![m] (C θ)) -∗ (∀R: θ, C θ) ≤ₜ ![m] (∀R: θ, C θ).
+  Proof. 
+    iIntros "#Hle % !# H". rewrite /sem_ty_mbang /sem_ty_row_forall.
+    iApply forall_intuitionistically_if. iIntros (ρ).
+    iApply ("Hle" with "H").
+  Qed.
+  
+  Global Instance multi_ty_row_forall (C : sem_row Σ → sem_ty Σ) `{! ∀ θ, MultiT (C θ) } : 
+    MultiT (∀R: θ, C θ).
+  Proof. 
+    constructor. iApply ty_le_mbang_intro_row_forall. 
+    iIntros (τ). specialize (H τ). inv H. iApply multi_ty0.
+  Qed.
+
+  Lemma ty_le_mbang_intro_mode_forall (C : mode → sem_ty Σ) m :
+    (∀ ν, (C ν) ≤ₜ ![m] (C ν)) -∗ (∀M: ν, C ν) ≤ₜ ![m] (∀M: ν, C ν).
+  Proof. 
+    iIntros "#Hle % !# H". rewrite /sem_ty_mbang /sem_ty_mode_forall.
+    iApply forall_intuitionistically_if. iIntros (m').
+    iApply ("Hle" with "H").
+  Qed.
+
+  Global Instance multi_ty_mode_forall (C : mode → sem_ty Σ) `{ ∀ ν, MultiT (C ν) } : 
+    MultiT (∀M: ν, C ν).
+  Proof. 
+    constructor. iApply ty_le_mbang_intro_mode_forall. 
+    iIntros (τ). specialize (H τ). inv H. iApply multi_ty0.
+  Qed.
+
+  Lemma ty_le_mbang_intro_ref_cpy τ m : ⊢ (Refᶜ τ) ≤ₜ ![m] (Refᶜ τ).
+  Proof. 
+    iIntros "!# % #H". 
+    iApply bi.intuitionistically_intuitionistically_if. 
+    iIntros "!# //".
+  Qed.
+
+  Global Instance multi_ty_ref_cpy τ : MultiT (Refᶜ τ).
+  Proof. constructor. iApply ty_le_mbang_intro_ref_cpy. Qed.
+
+  Lemma ty_le_mbang_intro_exists A m : (∀ α, (A α) ≤ₜ ![m] (A α)) -∗ (∃: α, A α) ≤ₜ ![m] (∃: α, A α).
+  Proof. 
+    iIntros "#H !# % [%α Hτ']". 
+    iDestruct ("H" with "Hτ'") as "Hτ".
+    iApply (bi.intuitionistically_if_mono with "Hτ").
+    iIntros "HA". by iExists α.
+  Qed.
+
+  Global Instance multi_ty_exists A `{ ∀ α, MultiT (A α) } : MultiT (∃: α, A α).
+  Proof. 
+    constructor. iApply ty_le_mbang_intro_exists.
+    iIntros (τ). specialize (H τ). inv H. iApply multi_ty0.
+  Qed.
+
+  Corollary ty_le_mbang_intro_option τ m : τ ≤ₜ ![m] τ -∗ (Option τ) ≤ₜ ![m] (Option τ).
   Proof. 
     iIntros "#H". 
-    destruct m; simpl; first iApply ty_le_refl.
+    iApply ty_le_mbang_intro_sum; [iApply ty_le_mbang_intro_unit|done]. 
+  Qed.
+
+  Corollary multi_ty_option τ `{! MultiT τ } : MultiT (Option τ). 
+  Proof. apply _. Qed. 
+
+  Lemma ty_le_mbang_intro_rec m (C : sem_ty Σ → sem_ty Σ) `{NonExpansive C} :
+    □ (∀ α, (α ≤ₜ ![m] α) -∗ C α ≤ₜ ![m] (C α)) -∗
+    (μT: α, C α) ≤ₜ ![m] (μT: α, C α).
+  Proof. 
+    iIntros "#H". destruct m; simpl; first iApply ty_le_refl.
     iIntros "!# %v Hτα".
     iLöb as "IH" forall (v).
     rewrite {1} sem_ty_rec_unfold.
-    assert (fixpoint (sem_ty_rec_pre τ) v ≡ sem_ty_rec_pre τ (fixpoint (sem_ty_rec_pre τ)) v).
+    assert (fixpoint (sem_ty_rec_pre C) v ≡ sem_ty_rec_pre C (fixpoint (sem_ty_rec_pre C)) v).
     { apply non_dep_fun_equiv. apply fixpoint_unfold. }
-    rewrite {4} /sem_ty_rec /sem_ty_bang H {1} /sem_ty_rec_pre.
-    iApply bi.later_intuitionistically. iNext. iExists (fixpoint (sem_ty_rec_pre τ)).
-    iSpecialize ("H" $! (μT: α, τ α)%T with "[IH]").
+    rewrite {4} /sem_ty_rec /sem_ty_mbang H {1} /sem_ty_rec_pre. simpl.
+    iApply bi.later_intuitionistically. iNext. iExists (fixpoint (sem_ty_rec_pre C)).
+    iSpecialize ("H" $! (μT: α, C α)%T with "[IH]").
     { iIntros "% !# //". }
     iDestruct ("H" $! v with "Hτα") as "#Hτα'". iIntros "!#".
     iSplit; first done. iApply "Hτα'".
   Qed.
 
-  Lemma ty_le_list (τ₁ τ₂ : sem_ty Σ) :
-    τ₁ ≤T τ₂ -∗
-    List τ₁ ≤T List τ₂.
-  Proof.
-    iIntros "#Hτ₁₂ !# %v HLτ₁". unfold sem_ty_list.
-    iLöb as "IH" forall (v).
-    iApply sem_ty_rec_unfold.
-    rewrite sem_ty_rec_unfold. iNext.
-    iDestruct "HLτ₁" as "(%v' & [(-> & Hunit)|(-> & (%w₁ & %w₂ & -> & Hτ₁ & Hμ))])".
-    { iExists v'; iLeft. by iFrame. }
-    iExists (w₁, w₂)%V. iRight. iSplit; first done.
-    iExists w₁, w₂; iSplit; first done.
-    iSplitL "Hτ₁"; [by iApply "Hτ₁₂"|by iApply "IH"].
+  (* The premise uses the unfolded ty_le definition instead of MultiT because it lives in iProp.
+     As a result, to prove MultiT for rec types we have to manually prove the instance 
+     using the ty_le_mbang_intro_* instances *)
+  Global Instance multi_ty_rec (C : sem_ty Σ → sem_ty Σ) `{NonExpansive C} : 
+    (∀ α, (α ≤ₜ ![MS] α) -∗ C α ≤ₜ ![MS] (C α)) →
+    MultiT (μT: α, C α).
+  Proof. 
+    constructor. iApply ty_le_mbang_intro_rec. 
+    iIntros "!# % H". specialize (H α).
+    by iApply H.
   Qed.
 
-  Lemma ty_le_list_bang m (τ : sem_ty Σ) :
-    ⊢ List ('!_[m] τ) ≤T '!_[m] (List ('!_[m] τ)).
+  Corollary ty_le_mbang_intro_list τ m : τ ≤ₜ ![m] τ -∗ (List τ) ≤ₜ ![m] (List τ).
   Proof.
-    rewrite /sem_ty_list /ListF. iIntros.
-    iApply ty_le_rec_bang. iIntros "!# %α #Hle".
-    iApply ty_le_mbang_sum_intro.
-    { iApply ty_le_mbang_intro. iApply copy_ty_unit. }
-    iApply (ty_le_mbang_prod_intro with "[] Hle").
-    iApply ty_le_mbang_idemp.
+    iIntros "#Hτ". iApply ty_le_mbang_intro_rec.
+    iIntros "!# % #Hα". 
+    iApply ty_le_mbang_intro_sum; [iApply ty_le_mbang_intro_unit|].
+    by iApply ty_le_mbang_intro_prod.
   Qed.
+
+  Global Instance multi_ty_list τ `{! MultiT τ } : MultiT (List τ).
+  Proof. constructor. inv MultiT0. by iApply ty_le_mbang_intro_list. Qed.
+
+  Lemma ty_le_mbang_elim (m : mode) (τ : sem_ty Σ) :
+    ⊢ (![m] τ) ≤ₜ τ.
+  Proof. iIntros "!# % H". iDestruct (bi.intuitionistically_if_elim with "H") as "$". Qed.
+
+  Lemma ty_le_mbang_comp m m' (τ τ' : sem_ty Σ) :
+    m' ≤ₘ m -∗ τ ≤ₜ τ' -∗ 
+    (![m] τ) ≤ₜ (![m'] τ').
+  Proof. 
+    iIntros "#Hmm' #Hττ'". 
+    iIntros "!# % Hτ". destruct m.
+    - iDestruct (mode_le_OS_inv with "Hmm'") as "->".
+      rewrite /sem_ty_mbang /=. by iApply "Hττ'".
+    - rewrite /sem_ty_mbang /=. iDestruct "Hτ" as "#Hτ".
+      iApply bi.intuitionistically_intuitionistically_if. iIntros "!#".
+      by iApply "Hττ'". 
+  Qed.
+
+  Lemma ty_le_mbang_comm m m' (τ : sem_ty Σ) :
+    ⊢ ![m] (![m'] τ) ≤ₜ ![m'] (![m] τ). 
+  Proof.
+    destruct m, m'.
+    - iApply ty_le_refl.
+    - iApply ty_le_trans; first iApply ty_le_mbang_elim. 
+      iApply ty_le_mbang_comp.
+      { iApply mode_le_refl. }
+      iApply ty_le_mbang_intro_os.
+    - iApply ty_le_trans; first iApply ty_le_mbang_comp.
+      { iApply mode_le_refl. }
+      { iApply ty_le_mbang_elim. }
+      iApply ty_le_mbang_intro_os.
+    - iApply ty_le_refl.
+  Qed.
+
+  Lemma ty_le_mbang_type_forall (C : sem_ty Σ → sem_ty Σ) m :
+    ⊢ (∀T: α, ![m] (C α))%T ≤ₜ ![m] (∀T: α, C α).
+  Proof. 
+    iIntros "!# %v Hτ". 
+    iApply forall_intuitionistically_if. iIntros (τ).
+    iApply "Hτ".
+  Qed.
+
+  Lemma ty_le_type_forall_mbang (C : sem_ty Σ → sem_ty Σ) m :
+    ⊢ ![m] (∀T: α, C α) ≤ₜ (∀T: α, ![m] (C α))%T.
+  Proof. 
+    iIntros "!# %v Hτ".  
+    iDestruct (intuitionistically_if_forall with "Hτ") as "Hτ". 
+    iApply "Hτ".
+  Qed.
+
+  Lemma ty_le_mbang_row_forall (C : sem_row Σ → sem_ty Σ) m :
+    ⊢ (∀R: θ, ![m] (C θ))%T ≤ₜ ![m] (∀R: θ, C θ).
+  Proof. 
+    iIntros "!# %v Hτ". 
+    iApply forall_intuitionistically_if. iIntros (τ).
+    iApply "Hτ".
+  Qed.
+
+  Lemma ty_le_row_forall_mbang (C : sem_row Σ → sem_ty Σ) m :
+    ⊢ ![m] (∀R: θ, C θ) ≤ₜ (∀R: θ, ![m] (C θ))%T.
+  Proof. 
+    iIntros "!# %v Hτ".  
+    iDestruct (intuitionistically_if_forall with "Hτ") as "Hτ". 
+    iApply "Hτ".
+  Qed.
+
+  Lemma ty_le_mbang_mode_forall (C : mode → sem_ty Σ) m :
+    ⊢ (∀M: ν, ![m] (C ν))%T ≤ₜ ![m] (∀M: ν, C ν).
+  Proof. 
+    iIntros "!# %v Hτ". 
+    iApply forall_intuitionistically_if. iIntros (τ).
+    iApply "Hτ".
+  Qed.
+
+  Lemma ty_le_mode_forall_mbang (C : mode → sem_ty Σ) m :
+    ⊢ ![m] (∀M: ν, C ν) ≤ₜ (∀M: ν, ![m] (C ν))%T.
+  Proof. 
+    iIntros "!# %v Hτ".  
+    iDestruct (intuitionistically_if_forall with "Hτ") as "Hτ". 
+    iApply "Hτ".
+  Qed.
+
+  Corollary ty_le_uarr (τ₁ κ₁ τ₂ κ₂ : sem_ty Σ) (ρ ρ' : sem_row Σ) :
+    ρ ≤ᵣ ρ' -∗
+    τ₂ ≤ₜ τ₁ -∗
+    κ₁ ≤ₜ κ₂ -∗
+    (τ₁ -{ ρ }-> κ₁) ≤ₜ (τ₂ -{ ρ' }-> κ₂).
+  Proof.
+    iIntros "#Hρ  #Hτ₂₁ #Hκ₁₂". 
+    iApply ty_le_mbang_comp; first iApply mode_le_refl. 
+    by iApply ty_le_arr.
+  Qed.
+      
+  Corollary ty_le_u2aarr (τ κ : sem_ty Σ) (ρ : sem_row Σ) :
+    ⊢ (τ -{ ρ }-> κ) ≤ₜ (τ -{ ρ }-∘ κ).
+  Proof. apply ty_le_mbang_elim. Qed.
+
 End sub_typing.
+
+Section row_type_sub.
+
+  (* Subsumption relation on rows wrt to types *)
+  
+  Global Instance row_type_sub_multi_ty {Σ} (ρ : sem_row Σ) (τ : sem_ty Σ) `{! MultiT τ} : ρ ᵣ⪯ₜ τ.
+  Proof.
+    constructor.
+    iIntros "%w %v %Φ !# Hρ #Hτ".
+    iApply (pmono_prot_prop _ (sem_row_car ρ) with "[] Hρ").
+    iIntros "!# % H". iFrame. rewrite /sem_ty_mbang /= //.
+  Qed.
+  
+  Global Instance row_type_sub_mfbang_mbang {Σ} (m : mode) (ρ : sem_row Σ) (τ : sem_ty Σ) : ¡[ m ] ρ ᵣ⪯ₜ (![ m ] τ).
+  Proof. 
+    destruct m; first apply _. 
+    apply row_type_sub_multi_ty. apply _.
+  Qed.
+  
+End row_type_sub.
+
+Section mode_type_sub.
+
+  (* Subsumption relation on modes wrt to types *)
+
+  Global Instance mode_type_sub_multi_ty {Σ} m (τ : sem_ty Σ) `{! MultiT τ } : m ₘ⪯ₜ τ.
+  Proof. 
+    constructor. iIntros "% #Hτ". 
+    by iApply bi.intuitionistically_intuitionistically_if.
+  Qed.
+
+  Global Instance mode_type_sub_mbang {Σ} m (τ : sem_ty Σ) : m ₘ⪯ₜ (![m] τ).
+  Proof. 
+    constructor. iIntros "% Hτ". 
+    iApply bi.intuitionistically_if_idemp. iApply "Hτ".
+  Qed.
+  
+End mode_type_sub.
